@prefix dc: <http://purl.org/dc/elements/1.1/> .
@prefix dcam: <http://purl.org/dc/dcam/> .
@prefix dcmitype: <http://purl.org/dc/dcmitype/> .
@prefix dcterms: <http://purl.org/dc/terms/> .
@prefix foaf: <http://xmlns.com/foaf/0.1/> .
@prefix owl: <http://www.w3.org/2002/07/owl#> .
@prefix rdf: <http://www.w3.org/1999/02/22-rdf-syntax-ns#> .
@prefix rdfs: <http://www.w3.org/2000/01/rdf-schema#> .
@prefix skos: <http://www.w3.org/2004/02/skos/core#> .
@prefix xsd: <http://www.w3.org/2001/XMLSchema#> .

dcterms:Agent a dcterms:AgentClass,
        rdfs:Class ;
    rdfs:label "Agent"@en ;
    dcterms:issued "2008-01-14"^^xsd:date ;
    rdfs:comment "A resource that acts or has the power to act."@en ;
    rdfs:isDefinedBy dcterms: ;
    skos:definition "موارد تمتلك القدرة على الفعل أو التصرف."@arabic ;
    skos:prefLabel "وكيل"@arabic .

dcterms:AgentClass a rdfs:Class ;
    rdfs:label "Agent Class"@en ;
    dcterms:issued "2008-01-14"^^xsd:date ;
    rdfs:comment "A group of agents."@en ;
    rdfs:isDefinedBy dcterms: ;
    rdfs:subClassOf rdfs:Class ;
    skos:definition "مجموعة من الوكلاء"@arabic ;
    skos:prefLabel "فئة الوكيل"@arabic .

dcterms:BibliographicResource a rdfs:Class ;
    rdfs:label "Bibliographic Resource"@en ;
    dcterms:issued "2008-01-14"^^xsd:date ;
    rdfs:comment "A book, article, or other documentary resource."@en ;
    rdfs:isDefinedBy dcterms: ;
    skos:definition "مصدر وثائقي يتضمن كتابًا أو مقالة أو أي مادة مكتوبة أو منشورة أخرى."@arabic ;
    skos:prefLabel "مصدر ببليوغرافي"@arabic .

dcterms:FileFormat a rdfs:Class ;
    rdfs:label "File Format"@en ;
    dcterms:issued "2008-01-14"^^xsd:date ;
    rdfs:comment "A digital resource format."@en ;
    rdfs:isDefinedBy dcterms: ;
    rdfs:subClassOf dcterms:MediaType ;
    skos:definition "هي تنسيق رقمي يُستخدم لتخزين أو نقل الموارد الرقمية مثل النصوص والصور والفيديوهات."@arabic ;
    skos:prefLabel "تنسيق الملف"@arabic .

dcterms:Frequency a rdfs:Class ;
    rdfs:label "Frequency"@en ;
    dcterms:issued "2008-01-14"^^xsd:date ;
    rdfs:comment "A rate at which something recurs."@en ;
    rdfs:isDefinedBy dcterms: ;
    skos:definition "معدل حدوث شيء ما بصورة متكررة."@arabic ;
    skos:prefLabel "التردد"@arabic .

dcterms:Jurisdiction a rdfs:Class ;
    rdfs:label "Jurisdiction"@en ;
    dcterms:issued "2008-01-14"^^xsd:date ;
    rdfs:comment "The extent or range of judicial, law enforcement, or other authority."@en ;
    rdfs:isDefinedBy dcterms: ;
    rdfs:subClassOf dcterms:LocationPeriodOrJurisdiction ;
    skos:definition "مدى أو نطاق السلطة القضائية أو إنفاذ القانون أو أي سلطة أخرى."@arabic ;
    skos:prefLabel "الاختصاص"@arabic .

dcterms:LicenseDocument a rdfs:Class ;
    rdfs:label "License Document"@en ;
    dcterms:issued "2008-01-14"^^xsd:date ;
    rdfs:comment "A legal document giving official permission to do something with a resource."@en ;
    rdfs:isDefinedBy dcterms: ;
    rdfs:subClassOf dcterms:RightsStatement ;
    skos:definition "وثيقة قانونية تُمنح بها إذنًا رسميًا للقيام بشيء ما باستخدام مورد."@arabic ;
    skos:prefLabel "وثيقة الترخيص"@arabic .

dcterms:LinguisticSystem a rdfs:Class ;
    rdfs:label "Linguistic System"@en ;
    dcterms:description "Written, spoken, sign, and computer languages are linguistic systems."@en ;
    dcterms:issued "2008-01-14"^^xsd:date ;
    rdfs:comment "A system of signs, symbols, sounds, gestures, or rules used in communication."@en ;
    rdfs:isDefinedBy dcterms: ;
    skos:definition "نظام من العلامات أو الرموز أو الأصوات أو الإيماءات أو القواعد المستخدمة في التواصل."@arabic ;
    skos:prefLabel "النظام اللغوي"@arabic .

dcterms:Location a rdfs:Class ;
    rdfs:label "Location"@en ;
    dcterms:issued "2008-01-14"^^xsd:date ;
    rdfs:comment "A spatial region or named place."@en ;
    rdfs:isDefinedBy dcterms: ;
    rdfs:subClassOf dcterms:LocationPeriodOrJurisdiction ;
    skos:definition "منطقة فضائية أو مكان مسمى."@arabic ;
    skos:prefLabel "الموقع"@arabic .

dcterms:LocationPeriodOrJurisdiction a rdfs:Class ;
    rdfs:label "Location, Period, or Jurisdiction"@en ;
    dcterms:issued "2008-01-14"^^xsd:date ;
    rdfs:comment "A location, period of time, or jurisdiction."@en ;
    rdfs:isDefinedBy dcterms: ;
    skos:definition "مكان أو فترة زمنية أو نطاق قضائي"@arabic ;
    skos:prefLabel "الموقع، الفترة، أو الولاية القضائية"@arabic .

dcterms:MediaType a rdfs:Class ;
    rdfs:label "Media Type"@en ;
    dcterms:issued "2008-01-14"^^xsd:date ;
    rdfs:comment "A file format or physical medium."@en ;
    rdfs:isDefinedBy dcterms: ;
    rdfs:subClassOf dcterms:MediaTypeOrExtent ;
    skos:definition "هي صيغة تُستخدم لتخزين البيانات على شكل ملف أو وسيط مادي، وتحدد تنظيم وترميز المعلومات في هذا الوسيط."@arabic ;
    skos:prefLabel "نوع الوسائط"@arabic .

dcterms:MediaTypeOrExtent a rdfs:Class ;
    rdfs:label "Media Type or Extent"@en ;
    dcterms:issued "2008-01-14"^^xsd:date ;
    rdfs:comment "A media type or extent."@en ;
    rdfs:isDefinedBy dcterms: ;
    skos:definition "الوسائط أو الامتداد: مصطلح يُستخدم للإشارة إلى صيغة أو تنسيق محتوى رقمي، يحدد طريقة تعريف ومعالجة هذا المحتوى في الأنظمة والبرامج."@arabic ;
    skos:prefLabel "نوع الوسائط أو المدى"@arabic .

dcterms:MethodOfAccrual a rdfs:Class ;
    rdfs:label "Method of Accrual"@en ;
    dcterms:issued "2008-01-14"^^xsd:date ;
    rdfs:comment "A method by which resources are added to a collection."@en ;
    rdfs:isDefinedBy dcterms: ;
    skos:definition "طريقة تُستخدم لإضافة موارد إلى مجموعة معينة، وتُعنى بدمج أو تجميع الموارد أو العناصر في مجموعة محددة."@arabic ;
    skos:prefLabel "طريقة الاستحقاق"@arabic .

dcterms:MethodOfInstruction a rdfs:Class ;
    rdfs:label "Method of Instruction"@en ;
    dcterms:issued "2008-01-14"^^xsd:date ;
    rdfs:comment "A process that is used to engender knowledge, attitudes, and skills."@en ;
    rdfs:isDefinedBy dcterms: ;
    skos:definition "عملية تُستخدم لتوليد أو اكتساب المعرفة والمواقف والمهارات."@arabic ;
    skos:prefLabel "طريقة التدريس"@arabic .

dcterms:PeriodOfTime a rdfs:Class ;
    rdfs:label "Period of Time"@en ;
    dcterms:issued "2008-01-14"^^xsd:date ;
    rdfs:comment "An interval of time that is named or defined by its start and end dates."@en ;
    rdfs:isDefinedBy dcterms: ;
    rdfs:subClassOf dcterms:LocationPeriodOrJurisdiction ;
    skos:definition "فترة زمنية تُعرَّف أو تُسمَّى بواسطة تاريخي البدء والنهاية."@arabic ;
    skos:prefLabel "فترة زمنية"@arabic .

dcterms:PhysicalMedium a rdfs:Class ;
    rdfs:label "Physical Medium"@en ;
    dcterms:description "Examples include paper, canvas, or DVD."@en ;
    dcterms:issued "2008-01-14"^^xsd:date ;
    rdfs:comment "A physical material or carrier."@en ;
    rdfs:isDefinedBy dcterms: ;
    rdfs:subClassOf dcterms:MediaType ;
    skos:definition "مادة فعلية أو وسيلة لنقل شيء ما."@arabic ;
    skos:prefLabel "الوسط المادي"@arabic .

dcterms:PhysicalResource a rdfs:Class ;
    rdfs:label "Physical Resource"@en ;
    dcterms:issued "2008-01-14"^^xsd:date ;
    rdfs:comment "A material thing."@en ;
    rdfs:isDefinedBy dcterms: ;
    skos:definition "شيء ملموس يتكوّن من مادة."@arabic ;
    skos:prefLabel "المورد المادي"@arabic .

dcterms:Policy a rdfs:Class ;
    rdfs:label "Policy"@en ;
    dcterms:issued "2008-01-14"^^xsd:date ;
    rdfs:comment "A plan or course of action by an authority, intended to influence and determine decisions, actions, and other matters."@en ;
    rdfs:isDefinedBy dcterms: ;
    skos:definition "خطة أو مسار عمل يُضعه سلطة تهدف إلى التأثير في اتخاذ القرارات وتحديد الإجراءات والمسائل الأخرى."@arabic ;
    skos:prefLabel "سياسة"@arabic .

dcterms:ProvenanceStatement a rdfs:Class ;
    rdfs:label "Provenance Statement"@en ;
    dcterms:issued "2008-01-14"^^xsd:date ;
    rdfs:comment "Any changes in ownership and custody of a resource since its creation that are significant for its authenticity, integrity, and interpretation."@en ;
    rdfs:isDefinedBy dcterms: ;
    skos:definition "أي تغيّر في ملكية أو حيازة مورد منذ إنشائه يُعدّ ذا أهمية كبيرة لتوثيقه، سلامته، وتفسيره."@arabic ;
    skos:prefLabel "بيان المنشأ"@arabic .

dcterms:RightsStatement a rdfs:Class ;
    rdfs:label "Rights Statement"@en ;
    dcterms:issued "2008-01-14"^^xsd:date ;
    rdfs:comment "A statement about the intellectual property rights (IPR) held in or over a resource, a legal document giving official permission to do something with a resource, or a statement about access rights."@en ;
    rdfs:isDefinedBy dcterms: ;
    skos:definition "بيان يوضح حقوق الملكية الفكرية (IPR) المملوكة أو المطبقة على مورد ما، أو وثيقة قانونية تمنح إذنًا رسميًا للقيام بشيء ما باستخدام المورد، أو بيان عن حقوق الوصول إلى المورد."@arabic ;
    skos:prefLabel "بيان الحقوق"@arabic .

dcterms:SizeOrDuration a rdfs:Class ;
    rdfs:label "Size or Duration"@en ;
    dcterms:description "Examples include a number of pages, a specification of length, width, and breadth, or a period in hours, minutes, and seconds."@en ;
    dcterms:issued "2008-01-14"^^xsd:date ;
    rdfs:comment "A dimension or extent, or a time taken to play or execute."@en ;
    rdfs:isDefinedBy dcterms: ;
    rdfs:subClassOf dcterms:MediaTypeOrExtent ;
    skos:definition "المدة الزمنية أو البُعد أو الفترة التي يستغرقها أداء أو تنفيذ شيء ما."@arabic ;
    skos:prefLabel "الحجم أو المدة"@arabic .

dcterms:Standard a rdfs:Class ;
    rdfs:label "Standard"@en ;
    dcterms:issued "2008-01-14"^^xsd:date ;
    rdfs:comment "A reference point against which other things can be evaluated or compared."@en ;
    rdfs:isDefinedBy dcterms: ;
    skos:definition "نقطة مرجعية تُستعمل لتقييم أو مقارنة أشياء أخرى."@arabic ;
    skos:prefLabel "القياسي"@arabic .

dcterms:Box a rdfs:Datatype ;
    rdfs:label "DCMI Box"@en ;
    dcterms:issued "2000-07-11"^^xsd:date ;
    rdfs:comment "The set of regions in space defined by their geographic coordinates according to the DCMI Box Encoding Scheme."@en ;
    rdfs:isDefinedBy dcterms: ;
    rdfs:seeAlso <https://www.dublincore.org/specifications/dublin-core/dcmi-box/> .

dcterms:DCMIType a dcam:VocabularyEncodingScheme ;
    rdfs:label "DCMI Type Vocabulary"@en ;
    dcterms:issued "2000-07-11"^^xsd:date ;
    rdfs:comment "The set of classes specified by the DCMI Type Vocabulary, used to categorize the nature or genre of the resource."@en ;
    rdfs:isDefinedBy dcterms: ;
    rdfs:seeAlso dcmitype: .

dcterms:DDC a dcam:VocabularyEncodingScheme ;
    rdfs:label "DDC"@en ;
    dcterms:issued "2000-07-11"^^xsd:date ;
    rdfs:comment "The set of conceptual resources specified by the Dewey Decimal Classification."@en ;
    rdfs:isDefinedBy dcterms: ;
    rdfs:seeAlso <http://www.oclc.org/dewey/> .

dcterms:IMT a dcam:VocabularyEncodingScheme ;
    rdfs:label "IMT"@en ;
    dcterms:issued "2000-07-11"^^xsd:date ;
    rdfs:comment "The set of media types specified by the Internet Assigned Numbers Authority."@en ;
    rdfs:isDefinedBy dcterms: ;
    rdfs:seeAlso <http://www.iana.org/assignments/media-types/> .

dcterms:ISO3166 a rdfs:Datatype ;
    rdfs:label "ISO 3166"@en ;
    dcterms:issued "2000-07-11"^^xsd:date ;
    rdfs:comment "The set of codes listed in ISO 3166-1 for the representation of names of countries."@en ;
    rdfs:isDefinedBy dcterms: ;
    rdfs:seeAlso <https://www.iso.org/obp/ui/#search> .

dcterms:ISO639-2 a rdfs:Datatype ;
    rdfs:label "ISO 639-2"@en ;
    dcterms:issued "2000-07-11"^^xsd:date ;
    rdfs:comment "The three-letter alphabetic codes listed in ISO639-2 for the representation of names of languages."@en ;
    rdfs:isDefinedBy dcterms: ;
    rdfs:seeAlso <http://lcweb.loc.gov/standards/iso639-2/langhome.html> .

dcterms:ISO639-3 a rdfs:Datatype ;
    rdfs:label "ISO 639-3"@en ;
    dcterms:issued "2008-01-14"^^xsd:date ;
    rdfs:comment "The set of three-letter codes listed in ISO 639-3 for the representation of names of languages."@en ;
    rdfs:isDefinedBy dcterms: ;
    rdfs:seeAlso <http://www.sil.org/iso639-3/> .

dcterms:LCC a dcam:VocabularyEncodingScheme ;
    rdfs:label "LCC"@en ;
    dcterms:issued "2000-07-11"^^xsd:date ;
    rdfs:comment "The set of conceptual resources specified by the Library of Congress Classification."@en ;
    rdfs:isDefinedBy dcterms: ;
    rdfs:seeAlso <http://lcweb.loc.gov/catdir/cpso/lcco/lcco.html> .

dcterms:LCSH a dcam:VocabularyEncodingScheme ;
    rdfs:label "LCSH"@en ;
    dcterms:issued "2000-07-11"^^xsd:date ;
    rdfs:comment "The set of labeled concepts specified by the Library of Congress Subject Headings."@en ;
    rdfs:isDefinedBy dcterms: .

dcterms:MESH a dcam:VocabularyEncodingScheme ;
    rdfs:label "MeSH"@en ;
    dcterms:issued "2000-07-11"^^xsd:date ;
    rdfs:comment "The set of labeled concepts specified by the Medical Subject Headings."@en ;
    rdfs:isDefinedBy dcterms: ;
    rdfs:seeAlso <http://www.nlm.nih.gov/mesh/meshhome.html> .

dcterms:NLM a dcam:VocabularyEncodingScheme ;
    rdfs:label "NLM"@en ;
    dcterms:issued "2005-06-13"^^xsd:date ;
    rdfs:comment "The set of conceptual resources specified by the National Library of Medicine Classification."@en ;
    rdfs:isDefinedBy dcterms: ;
    rdfs:seeAlso <http://wwwcf.nlm.nih.gov/class/> .

dcterms:Point a rdfs:Datatype ;
    rdfs:label "DCMI Point"@en ;
    dcterms:issued "2000-07-11"^^xsd:date ;
    rdfs:comment "The set of points in space defined by their geographic coordinates according to the DCMI Point Encoding Scheme."@en ;
    rdfs:isDefinedBy dcterms: ;
    rdfs:seeAlso <https://www.dublincore.org/specifications/dublin-core/dcmi-point/> .

dcterms:RFC1766 a rdfs:Datatype ;
    rdfs:label "RFC 1766"@en ;
    dcterms:issued "2000-07-11"^^xsd:date ;
    rdfs:comment "The set of tags, constructed according to RFC 1766, for the identification of languages."@en ;
    rdfs:isDefinedBy dcterms: ;
    rdfs:seeAlso <http://www.ietf.org/rfc/rfc1766.txt> .

dcterms:RFC3066 a rdfs:Datatype ;
    rdfs:label "RFC 3066"@en ;
    dcterms:description "RFC 3066 has been obsoleted by RFC 4646."@en ;
    dcterms:issued "2002-07-13"^^xsd:date ;
    rdfs:comment "The set of tags constructed according to RFC 3066 for the identification of languages."@en ;
    rdfs:isDefinedBy dcterms: ;
    rdfs:seeAlso <http://www.ietf.org/rfc/rfc3066.txt> .

dcterms:RFC4646 a rdfs:Datatype ;
    rdfs:label "RFC 4646"@en ;
    dcterms:description "RFC 4646 obsoletes RFC 3066."@en ;
    dcterms:issued "2008-01-14"^^xsd:date ;
    rdfs:comment "The set of tags constructed according to RFC 4646 for the identification of languages."@en ;
    rdfs:isDefinedBy dcterms: ;
    rdfs:seeAlso <http://www.ietf.org/rfc/rfc4646.txt> .

dcterms:RFC5646 a rdfs:Datatype ;
    rdfs:label "RFC 5646"@en ;
    dcterms:description "RFC 5646 obsoletes RFC 4646."@en ;
    dcterms:issued "2010-10-11"^^xsd:date ;
    rdfs:comment "The set of tags constructed according to RFC 5646 for the identification of languages."@en ;
    rdfs:isDefinedBy dcterms: ;
    rdfs:seeAlso <http://www.ietf.org/rfc/rfc5646.txt> .

dcterms:TGN a dcam:VocabularyEncodingScheme ;
    rdfs:label "TGN"@en ;
    dcterms:issued "2000-07-11"^^xsd:date ;
    rdfs:comment "The set of places specified by the Getty Thesaurus of Geographic Names."@en ;
    rdfs:isDefinedBy dcterms: ;
    rdfs:seeAlso <http://www.getty.edu/research/tools/vocabulary/tgn/index.html> .

dcterms:UDC a dcam:VocabularyEncodingScheme ;
    rdfs:label "UDC"@en ;
    dcterms:issued "2000-07-11"^^xsd:date ;
    rdfs:comment "The set of conceptual resources specified by the Universal Decimal Classification."@en ;
    rdfs:isDefinedBy dcterms: ;
    rdfs:seeAlso <http://www.udcc.org/> .

dcterms:URI a rdfs:Datatype ;
    rdfs:label "URI"@en ;
    dcterms:issued "2000-07-11"^^xsd:date ;
    rdfs:comment "The set of identifiers constructed according to the generic syntax for Uniform Resource Identifiers as specified by the Internet Engineering Task Force."@en ;
    rdfs:isDefinedBy dcterms: ;
    rdfs:seeAlso <http://www.ietf.org/rfc/rfc3986.txt> .

dcterms:W3CDTF a rdfs:Datatype ;
    rdfs:label "W3C-DTF"@en ;
    dcterms:issued "2000-07-11"^^xsd:date ;
    rdfs:comment "The set of dates and times constructed according to the W3C Date and Time Formats Specification."@en ;
    rdfs:isDefinedBy dcterms: ;
    rdfs:seeAlso <http://www.w3.org/TR/NOTE-datetime> .

dcterms:abstract a rdf:Property ;
    rdfs:label "Abstract"@en ;
    dcterms:issued "2000-07-11"^^xsd:date ;
    rdfs:comment "A summary of the resource."@en ;
    rdfs:isDefinedBy dcterms: ;
    rdfs:subPropertyOf dc:description,
        dcterms:description ;
    skos:definition "ملخّص للمصدر"@arabic ;
    skos:prefLabel "الملخص"@arabic .

dcterms:accessRights a rdf:Property ;
    rdfs:label "Access Rights"@en ;
    dcam:rangeIncludes dcterms:RightsStatement ;
    dcterms:description "Access Rights may include information regarding access or restrictions based on privacy, security, or other policies."@en ;
    dcterms:issued "2003-02-15"^^xsd:date ;
    rdfs:comment "Information about who access the resource or an indication of its security status."@en ;
    rdfs:isDefinedBy dcterms: ;
    rdfs:subPropertyOf dc:rights,
        dcterms:rights ;
    skos:definition "معلومات حول من يملك حق الوصول إلى المورد أو إشارة إلى حالته الأمنية."@arabic ;
    skos:prefLabel "حقوق الوصول"@arabic .

dcterms:accrualMethod a rdf:Property ;
    rdfs:label "Accrual Method"@en ;
    dcam:rangeIncludes dcterms:MethodOfAccrual ;
    dcterms:description "Recommended practice is to use a value from the Collection Description Accrual Method Vocabulary [[DCMI-ACCRUALMETHOD](https://dublincore.org/groups/collections/accrual-method/)]."@en ;
    dcterms:issued "2005-06-13"^^xsd:date ;
    rdfs:comment "The method by which items are added to a collection."@en ;
    rdfs:domain dcmitype:Collection ;
    rdfs:isDefinedBy dcterms: ;
    skos:definition "الطريقة التي تُضاف بها العناصر إلى مجموعة."@arabic ;
    skos:prefLabel "طريقة الاستحقاق"@arabic .

dcterms:accrualPeriodicity a rdf:Property ;
    rdfs:label "Accrual Periodicity"@en ;
    dcam:rangeIncludes dcterms:Frequency ;
    dcterms:description "Recommended practice is to use a value from the Collection Description Frequency Vocabulary [[DCMI-COLLFREQ](https://dublincore.org/groups/collections/frequency/)]."@en ;
    dcterms:issued "2005-06-13"^^xsd:date ;
    rdfs:comment "The frequency with which items are added to a collection."@en ;
    rdfs:domain dcmitype:Collection ;
    rdfs:isDefinedBy dcterms: ;
    skos:definition "معدل إضافة العناصر إلى مجموعة، أي التكرار الزمني الذي يتم فيه إضافة عناصر جديدة إلى المجموعة."@arabic ;
    skos:prefLabel "تكرار الاستحقاق"@arabic .

dcterms:accrualPolicy a rdf:Property ;
    rdfs:label "Accrual Policy"@en ;
    dcam:rangeIncludes dcterms:Policy ;
    dcterms:description "Recommended practice is to use a value from the Collection Description Accrual Policy Vocabulary [[DCMI-ACCRUALPOLICY](https://dublincore.org/groups/collections/accrual-policy/)]."@en ;
    dcterms:issued "2005-06-13"^^xsd:date ;
    rdfs:comment "The policy governing the addition of items to a collection."@en ;
    rdfs:domain dcmitype:Collection ;
    rdfs:isDefinedBy dcterms: ;
    skos:definition "سياسة تنظم إضافة العناصر إلى مجموعة."@arabic ;
    skos:prefLabel "سياسة الاستحقاق"@arabic .

dcterms:alternative a rdf:Property ;
    rdfs:label "Alternative Title"@en ;
    dcterms:description "The distinction between titles and alternative titles is application-specific."@en ;
    dcterms:issued "2000-07-11"^^xsd:date ;
    rdfs:comment "An alternative name for the resource."@en ;
    rdfs:isDefinedBy dcterms: ;
    rdfs:range rdfs:Literal ;
    rdfs:subPropertyOf dc:title,
        dcterms:title ;
    skos:definition "اسم بديل يُستخدم للإشارة إلى المورد بدلاً من اسمه الأصلي."@arabic ;
    skos:prefLabel "عنوان بديل"@arabic .

dcterms:available a rdf:Property ;
    rdfs:label "Date Available"@en ;
    dcterms:description "Recommended practice is to describe the date, date/time, or period of time as recommended for the property Date, of which this is a subproperty."@en ;
    dcterms:issued "2000-07-11"^^xsd:date ;
    rdfs:comment "Date that the resource became or will become available."@en ;
    rdfs:isDefinedBy dcterms: ;
    rdfs:range rdfs:Literal ;
    rdfs:subPropertyOf dc:date,
        dcterms:date ;
    skos:definition "التاريخ الذي يصبح فيه المورد متاحًا أو كان متاحًا."@arabic ;
    skos:prefLabel "التاريخ المتاح"@arabic .

dcterms:bibliographicCitation a rdf:Property ;
    rdfs:label "Bibliographic Citation"@en ;
    dcterms:description "Recommended practice is to include sufficient bibliographic detail to identify the resource as unambiguously as possible."@en ;
    dcterms:issued "2003-02-15"^^xsd:date ;
    rdfs:comment "A bibliographic reference for the resource."@en ;
    rdfs:isDefinedBy dcterms: ;
    rdfs:range rdfs:Literal ;
    rdfs:subPropertyOf dc:identifier,
        dcterms:identifier ;
    skos:definition "مرجع بُيُوغرافِيّ للموارد."@arabic ;
    skos:prefLabel "الاستشهاد الببليوغرافي"@arabic .

dcterms:conformsTo a rdf:Property ;
    rdfs:label "Conforms To"@en ;
    dcam:rangeIncludes dcterms:Standard ;
    dcterms:issued "2001-05-21"^^xsd:date ;
    rdfs:comment "An established standard to which the described resource conforms."@en ;
    rdfs:isDefinedBy dcterms: ;
    rdfs:subPropertyOf dc:relation,
        dcterms:relation ;
    skos:definition "معيار ثابت ومعتمد يلتزم به المورد المذكور."@arabic ;
    skos:prefLabel "متوافق مع"@arabic .

dcterms:created a rdf:Property ;
    rdfs:label "Date Created"@en ;
    dcterms:description "Recommended practice is to describe the date, date/time, or period of time as recommended for the property Date, of which this is a subproperty."@en ;
    dcterms:issued "2000-07-11"^^xsd:date ;
    rdfs:comment "Date of creation of the resource."@en ;
    rdfs:isDefinedBy dcterms: ;
    rdfs:range rdfs:Literal ;
    rdfs:subPropertyOf dc:date,
        dcterms:date ;
    skos:definition "تاريخ إنشاء المورد."@arabic ;
    skos:prefLabel "تاريخ الإنشاء"@arabic .

dcterms:creator a rdf:Property ;
    rdfs:label "Creator"@en ;
    dcam:rangeIncludes dcterms:Agent ;
    dcterms:description "Recommended practice is to identify the creator with a URI.  If this is not possible or feasible, a literal value that identifies the creator may be provided."@en ;
    dcterms:issued "2008-01-14"^^xsd:date ;
    rdfs:comment "An entity responsible for making the resource."@en ;
    rdfs:isDefinedBy dcterms: ;
    rdfs:subPropertyOf dc:creator,
        dcterms:contributor ;
    owl:equivalentProperty foaf:maker ;
    skos:definition "الكيان المسؤول عن إنتاج المورد."@arabic ;
    skos:prefLabel "المنشئ"@arabic .

dcterms:dateAccepted a rdf:Property ;
    rdfs:label "Date Accepted"@en ;
    dcterms:description "Recommended practice is to describe the date, date/time, or period of time as recommended for the property Date, of which this is a subproperty.  Examples of resources to which a date of acceptance may be relevant are a thesis (accepted by a university department) or an article (accepted by a journal)."@en ;
    dcterms:issued "2002-07-13"^^xsd:date ;
    rdfs:comment "Date of acceptance of the resource."@en ;
    rdfs:isDefinedBy dcterms: ;
    rdfs:range rdfs:Literal ;
    rdfs:subPropertyOf dc:date,
        dcterms:date ;
    skos:definition "التاريخ الذي يُسجَّل فيه قبول المورد من قبل الجهة المعنية."@arabic ;
    skos:prefLabel "تاريخ القبول"@arabic .

dcterms:dateCopyrighted a rdf:Property ;
    rdfs:label "Date Copyrighted"@en ;
    dcterms:description "Typically a year.  Recommended practice is to describe the date, date/time, or period of time as recommended for the property Date, of which this is a subproperty."@en ;
    dcterms:issued "2002-07-13"^^xsd:date ;
    rdfs:comment "Date of copyright of the resource."@en ;
    rdfs:isDefinedBy dcterms: ;
    rdfs:range rdfs:Literal ;
    rdfs:subPropertyOf dc:date,
        dcterms:date ;
    skos:definition "تاريخ تسجيل حقوق النشر للمصدر."@arabic ;
    skos:prefLabel "تاريخ حقوق النشر"@arabic .

dcterms:dateSubmitted a rdf:Property ;
    rdfs:label "Date Submitted"@en ;
    dcterms:description "Recommended practice is to describe the date, date/time, or period of time as recommended for the property Date, of which this is a subproperty.  Examples of resources to which a 'Date Submitted' may be relevant include a thesis (submitted to a university department) or an article (submitted to a journal)."@en ;
    dcterms:issued "2002-07-13"^^xsd:date ;
    rdfs:comment "Date of submission of the resource."@en ;
    rdfs:isDefinedBy dcterms: ;
    rdfs:range rdfs:Literal ;
    rdfs:subPropertyOf dc:date,
        dcterms:date ;
    skos:definition "تاريخ تقديم المورد"@arabic ;
    skos:prefLabel "التاريخ المُقدَّم"@arabic .

dcterms:educationLevel a rdf:Property ;
    rdfs:label "Audience Education Level"@en ;
    dcam:rangeIncludes dcterms:AgentClass ;
    dcterms:issued "2002-07-13"^^xsd:date ;
    rdfs:comment "A class of agents, defined in terms of progression through an educational or training context, for which the described resource is intended."@en ;
    rdfs:isDefinedBy dcterms: ;
    rdfs:subPropertyOf dcterms:audience ;
    skos:definition "فئة من الأفراد أو الكيانات تُعرَّف وفقًا لتقدمهم ضمن سياق تعليمي أو تدريبي، وتُستهدف بها الموارد الموصوفة."@arabic ;
    skos:prefLabel "مستوى تعليم الجمهور"@arabic .

dcterms:extent a rdf:Property ;
    rdfs:label "Extent"@en ;
    dcam:rangeIncludes dcterms:SizeOrDuration ;
    dcterms:description "Recommended practice is to specify the file size in megabytes and duration in ISO 8601 format."@en ;
    dcterms:issued "2000-07-11"^^xsd:date ;
    rdfs:comment "The size or duration of the resource."@en ;
    rdfs:isDefinedBy dcterms: ;
    rdfs:subPropertyOf dc:format,
        dcterms:format ;
    skos:definition "المقاس الذي يحدد حجم أو مدة المورد، سواء كان ذلك في مساحة أو زمن."@arabic ;
    skos:prefLabel "مدى"@arabic .

dcterms:hasFormat a rdf:Property ;
    rdfs:label "Has Format"@en ;
    dcterms:description "This property is intended to be used with non-literal values. This property is an inverse property of Is Format Of."@en ;
    dcterms:issued "2000-07-11"^^xsd:date ;
    rdfs:comment "A related resource that is substantially the same as the pre-existing described resource, but in another format."@en ;
    rdfs:isDefinedBy dcterms: ;
    rdfs:subPropertyOf dc:relation,
        dcterms:relation ;
    skos:definition "مورد مرتبط يختلف في الشكل فقط عن المورد الموصوف سابقًا، ويظل متشابهًا في المحتوى أو الفكرة الأساسية."@arabic ;
    skos:prefLabel "يحتوي على تنسيق"@arabic .

dcterms:hasPart a rdf:Property ;
    rdfs:label "Has Part"@en ;
    dcterms:description "This property is intended to be used with non-literal values. This property is an inverse property of Is Part Of."@en ;
    dcterms:issued "2000-07-11"^^xsd:date ;
    rdfs:comment "A related resource that is included either physically or logically in the described resource."@en ;
    rdfs:isDefinedBy dcterms: ;
    rdfs:subPropertyOf dc:relation,
        dcterms:relation ;
    skos:definition "مصدر ذي صلة يُدرج إما ماديًا أو منطقيًا داخل المورد المذكور."@arabic ;
    skos:prefLabel "يحتوي على جزء"@arabic .

dcterms:hasVersion a rdf:Property ;
    rdfs:label "Has Version"@en ;
    dcterms:description "Changes in version imply substantive changes in content rather than differences in format. This property is intended to be used with non-literal values. This property is an inverse property of Is Version Of."@en ;
    dcterms:issued "2000-07-11"^^xsd:date ;
    rdfs:comment "A related resource that is a version, edition, or adaptation of the described resource."@en ;
    rdfs:isDefinedBy dcterms: ;
    rdfs:subPropertyOf dc:relation,
        dcterms:relation ;
    skos:definition "المورد المرتبط هو نسخة أو إصدار أو تعديل من المورد المُوصف."@arabic ;
    skos:prefLabel "يحتوي على إصدار"@arabic .

dcterms:instructionalMethod a rdf:Property ;
    rdfs:label "Instructional Method"@en ;
    dcam:rangeIncludes dcterms:MethodOfInstruction ;
    dcterms:description "Instructional Method typically includes ways of presenting instructional materials or conducting instructional activities, patterns of learner-to-learner and learner-to-instructor interactions, and mechanisms by which group and individual levels of learning are measured.  Instructional methods include all aspects of the instruction and learning processes from planning and implementation through evaluation and feedback."@en ;
    dcterms:issued "2005-06-13"^^xsd:date ;
    rdfs:comment "A process, used to engender knowledge, attitudes and skills, that the described resource is designed to support."@en ;
    rdfs:isDefinedBy dcterms: ;
    skos:definition "عملية تُستخدم لتوليد المعرفة والمواقف والمهارات، ويُصمم المورد الموصوف لدعمها."@arabic ;
    skos:prefLabel "الطريقة التعليمية"@arabic .

dcterms:isFormatOf a rdf:Property ;
    rdfs:label "Is Format Of"@en ;
    dcterms:description "This property is intended to be used with non-literal values. This property is an inverse property of Has Format."@en ;
    dcterms:issued "2000-07-11"^^xsd:date ;
    rdfs:comment "A pre-existing related resource that is substantially the same as the described resource, but in another format."@en ;
    rdfs:isDefinedBy dcterms: ;
    rdfs:subPropertyOf dc:relation,
        dcterms:relation ;
    skos:definition "مورد مرتبط موجود مسبقاً يشبه إلى حد كبير المورد المذكور، ولكنه متاح في صيغة مختلفة."@arabic ;
    skos:prefLabel "هو تنسيق لـ"@arabic .

dcterms:isPartOf a rdf:Property ;
    rdfs:label "Is Part Of"@en ;
    dcterms:description "This property is intended to be used with non-literal values. This property is an inverse property of Has Part."@en ;
    dcterms:issued "2000-07-11"^^xsd:date ;
    rdfs:comment "A related resource in which the described resource is physically or logically included."@en ;
    rdfs:isDefinedBy dcterms: ;
    rdfs:subPropertyOf dc:relation,
        dcterms:relation ;
    skos:definition "مصدر مرتبط يكون المورد الموصوف متضمنًا فيه ماديًا أو منطقيًا."@arabic ;
    skos:prefLabel "جزء من"@arabic .

dcterms:isReferencedBy a rdf:Property ;
    rdfs:label "Is Referenced By"@en ;
    dcterms:description "This property is intended to be used with non-literal values. This property is an inverse property of References."@en ;
    dcterms:issued "2000-07-11"^^xsd:date ;
    rdfs:comment "A related resource that references, cites, or otherwise points to the described resource."@en ;
    rdfs:isDefinedBy dcterms: ;
    rdfs:subPropertyOf dc:relation,
        dcterms:relation ;
    skos:definition "موارد مرتبطة تُشير إلى أو تُستشهد بها أو تُوجه نحو المورد المُوصوف."@arabic ;
    skos:prefLabel "مُستشهد به"@arabic .

dcterms:isReplacedBy a rdf:Property ;
    rdfs:label "Is Replaced By"@en ;
    dcterms:description "This property is intended to be used with non-literal values. This property is an inverse property of Replaces."@en ;
    dcterms:issued "2000-07-11"^^xsd:date ;
    rdfs:comment "A related resource that supplants, displaces, or supersedes the described resource."@en ;
    rdfs:isDefinedBy dcterms: ;
    rdfs:subPropertyOf dc:relation,
        dcterms:relation ;
    skos:definition "مورد ذو صلة يُستبدل أو يُزاح أو يُفوق المورد الموصوف."@arabic ;
    skos:prefLabel "يستبدل بـ"@arabic .

dcterms:isRequiredBy a rdf:Property ;
    rdfs:label "Is Required By"@en ;
    dcterms:description "This property is intended to be used with non-literal values. This property is an inverse property of Requires."@en ;
    dcterms:issued "2000-07-11"^^xsd:date ;
    rdfs:comment "A related resource that requires the described resource to support its function, delivery, or coherence."@en ;
    rdfs:isDefinedBy dcterms: ;
    rdfs:subPropertyOf dc:relation,
        dcterms:relation ;
    skos:definition "مصدر مرتبط يتطلب وجود المورد المُصَفّ لدعم وظيفته أو تسليمه أو تماسكه."@arabic ;
    skos:prefLabel "مطلوب من"@arabic .

dcterms:isVersionOf a rdf:Property ;
    rdfs:label "Is Version Of"@en ;
    dcterms:description "Changes in version imply substantive changes in content rather than differences in format. This property is intended to be used with non-literal values. This property is an inverse property of Has Version."@en ;
    dcterms:issued "2000-07-11"^^xsd:date ;
    rdfs:comment "A related resource of which the described resource is a version, edition, or adaptation."@en ;
    rdfs:isDefinedBy dcterms: ;
    rdfs:subPropertyOf dc:relation,
        dcterms:relation ;
    skos:definition "مصدر متعلق يُعَدُّ فيه الموصوف نسخةً أو طبعةً أو تعديلاً لهذا المصدر."@arabic ;
    skos:prefLabel "هو إصدار من"@arabic .

dcterms:issued a rdf:Property ;
    rdfs:label "Date Issued"@en ;
    dcterms:description "Recommended practice is to describe the date, date/time, or period of time as recommended for the property Date, of which this is a subproperty."@en ;
    dcterms:issued "2000-07-11"^^xsd:date ;
    rdfs:comment "Date of formal issuance of the resource."@en ;
    rdfs:isDefinedBy dcterms: ;
    rdfs:range rdfs:Literal ;
    rdfs:subPropertyOf dc:date,
        dcterms:date ;
    skos:definition "التاريخ الذي يُصدر فيه المورد رسميًا، أي تاريخ إصدار الوثيقة أو العنصر وفقًا للسجلات الرسمية."@arabic ;
    skos:prefLabel "تاريخ الإصدار"@arabic .

dcterms:language a rdf:Property ;
    rdfs:label "Language"@en ;
    dcam:rangeIncludes dcterms:LinguisticSystem ;
    dcterms:description "Recommended practice is to use either a non-literal value representing a language from a controlled vocabulary such as ISO 639-2 or ISO 639-3, or a literal value consisting of an IETF Best Current Practice 47 [[IETF-BCP47](https://tools.ietf.org/html/bcp47)] language tag."@en ;
    dcterms:issued "2008-01-14"^^xsd:date ;
    rdfs:comment "A language of the resource."@en ;
    rdfs:isDefinedBy dcterms: ;
    rdfs:subPropertyOf dc:language ;
    skos:definition "اللغة المستخدمة لتحديد أو وصف المورد."@arabic ;
    skos:prefLabel "اللغة"@arabic .

dcterms:license a rdf:Property ;
    rdfs:label "License"@en ;
    dcam:rangeIncludes dcterms:LicenseDocument ;
    dcterms:description "Recommended practice is to identify the license document with a URI. If this is not possible or feasible, a literal value that identifies the license may be provided."@en ;
    dcterms:issued "2004-06-14"^^xsd:date ;
    rdfs:comment "A legal document giving official permission to do something with the resource."@en ;
    rdfs:isDefinedBy dcterms: ;
    rdfs:subPropertyOf dc:rights,
        dcterms:rights ;
    skos:definition "وثيقة قانونية تمنح الإذن الرسمي للقيام بعمل معيّن على المورد."@arabic ;
    skos:prefLabel "رخصة"@arabic .

dcterms:mediator a rdf:Property ;
    rdfs:label "Mediator"@en ;
    dcam:rangeIncludes dcterms:AgentClass ;
    dcterms:description "In an educational context, a mediator might be a parent, teacher, teaching assistant, or care-giver."@en ;
    dcterms:issued "2001-05-21"^^xsd:date ;
    rdfs:comment "An entity that mediates access to the resource."@en ;
    rdfs:isDefinedBy dcterms: ;
    rdfs:subPropertyOf dcterms:audience ;
    skos:definition "كيان يتوسط في الوصول إلى المورد."@arabic ;
    skos:prefLabel "وسيط"@arabic .

dcterms:medium a rdf:Property ;
    rdfs:label "Medium"@en ;
    dcam:domainIncludes dcterms:PhysicalResource ;
    dcam:rangeIncludes dcterms:PhysicalMedium ;
    dcterms:issued "2000-07-11"^^xsd:date ;
    rdfs:comment "The material or physical carrier of the resource."@en ;
    rdfs:isDefinedBy dcterms: ;
    rdfs:subPropertyOf dc:format,
        dcterms:format ;
    skos:definition "المادة أو الحامل الفيزيائي الذي يحمل المورد."@arabic ;
    skos:prefLabel "متوسط"@arabic .

dcterms:modified a rdf:Property ;
    rdfs:label "Date Modified"@en ;
    dcterms:description "Recommended practice is to describe the date, date/time, or period of time as recommended for the property Date, of which this is a subproperty."@en ;
    dcterms:issued "2000-07-11"^^xsd:date ;
    rdfs:comment "Date on which the resource was changed."@en ;
    rdfs:isDefinedBy dcterms: ;
    rdfs:range rdfs:Literal ;
    rdfs:subPropertyOf dc:date,
        dcterms:date ;
    skos:definition "التاريخ الذي تم فيه تعديل المورد."@arabic ;
    skos:prefLabel "تاريخ التعديل"@arabic .

dcterms:provenance a rdf:Property ;
    rdfs:label "Provenance"@en ;
    dcam:rangeIncludes dcterms:ProvenanceStatement ;
    dcterms:description "The statement may include a description of any changes successive custodians made to the resource."@en ;
    dcterms:issued "2004-09-20"^^xsd:date ;
    rdfs:comment "A statement of any changes in ownership and custody of the resource since its creation that are significant for its authenticity, integrity, and interpretation."@en ;
    rdfs:isDefinedBy dcterms: ;
    skos:definition "بيان عن أي تغييرات في الملكية والحضانة للموارِد منذ إنشائها، تُعَدّ مهمة لأصالتها وسلامتها وتفسيرها."@arabic ;
    skos:prefLabel "الأصل"@arabic .

dcterms:publisher a rdf:Property ;
    rdfs:label "Publisher"@en ;
    dcam:rangeIncludes dcterms:Agent ;
    dcterms:issued "2008-01-14"^^xsd:date ;
    rdfs:comment "An entity responsible for making the resource available."@en ;
    rdfs:isDefinedBy dcterms: ;
    rdfs:subPropertyOf dc:publisher ;
    skos:definition "الجهة المسؤولة عن جعل المورد متاحًا."@arabic ;
    skos:prefLabel "الناشر"@arabic .

dcterms:references a rdf:Property ;
    rdfs:label "References"@en ;
    dcterms:description "This property is intended to be used with non-literal values. This property is an inverse property of Is Referenced By."@en ;
    dcterms:issued "2000-07-11"^^xsd:date ;
    rdfs:comment "A related resource that is referenced, cited, or otherwise pointed to by the described resource."@en ;
    rdfs:isDefinedBy dcterms: ;
    rdfs:subPropertyOf dc:relation,
        dcterms:relation ;
    skos:definition "مصدر مرتبط يُستشهد به أو يُشار إليه أو يُنْشَر به بطريقة ما من قبل المورد المُوصوف."@arabic ;
    skos:prefLabel "المراجع"@arabic .

dcterms:replaces a rdf:Property ;
    rdfs:label "Replaces"@en ;
    dcterms:description "This property is intended to be used with non-literal values. This property is an inverse property of Is Replaced By."@en ;
    dcterms:issued "2000-07-11"^^xsd:date ;
    rdfs:comment "A related resource that is supplanted, displaced, or superseded by the described resource."@en ;
    rdfs:isDefinedBy dcterms: ;
    rdfs:subPropertyOf dc:relation,
        dcterms:relation ;
    skos:definition "مورد مرتبط يتم استبداله أو إزاحته أو تحقيره بالمورد المُوصف."@arabic ;
    skos:prefLabel "يستبدل"@arabic .

dcterms:requires a rdf:Property ;
    rdfs:label "Requires"@en ;
    dcterms:description "This property is intended to be used with non-literal values. This property is an inverse property of Is Required By."@en ;
    dcterms:issued "2000-07-11"^^xsd:date ;
    rdfs:comment "A related resource that is required by the described resource to support its function, delivery, or coherence."@en ;
    rdfs:isDefinedBy dcterms: ;
    rdfs:subPropertyOf dc:relation,
        dcterms:relation ;
    skos:definition "موارد ذات علاقة مطلوبة من قبل المورد المذكور لدعم وظيفته، أو تسليمه، أو توحيد عمله."@arabic ;
    skos:prefLabel "يتطلب"@arabic .

dcterms:rightsHolder a rdf:Property ;
    rdfs:label "Rights Holder"@en ;
    dcam:rangeIncludes dcterms:Agent ;
    dcterms:description "Recommended practice is to refer to the rights holder with a URI. If this is not possible or feasible, a literal value that identifies the rights holder may be provided."@en ;
    dcterms:issued "2004-06-14"^^xsd:date ;
    rdfs:comment "A person or organization owning or managing rights over the resource."@en ;
    rdfs:isDefinedBy dcterms: ;
    skos:definition "شخص أو منظمة تمتلك أو تدير حقوقًا على المورد."@arabic ;
    skos:prefLabel "صاحب الحقوق"@arabic .

dcterms:source a rdf:Property ;
    rdfs:label "Source"@en ;
    dcterms:description "This property is intended to be used with non-literal values. The described resource may be derived from the related resource in whole or in part. Best practice is to identify the related resource by means of a URI or a string conforming to a formal identification system."@en ;
    dcterms:issued "2008-01-14"^^xsd:date ;
    rdfs:comment "A related resource from which the described resource is derived."@en ;
    rdfs:isDefinedBy dcterms: ;
    rdfs:subPropertyOf dc:source,
        dcterms:relation ;
    skos:definition "مصدر ذو علاقة يُستمد منه المورد الموصوف."@arabic ;
    skos:prefLabel "مصدر"@arabic .

dcterms:spatial a rdf:Property ;
    rdfs:label "Spatial Coverage"@en ;
    dcam:rangeIncludes dcterms:Location ;
    dcterms:issued "2000-07-11"^^xsd:date ;
    rdfs:comment "Spatial characteristics of the resource."@en ;
    rdfs:isDefinedBy dcterms: ;
    rdfs:subPropertyOf dc:coverage,
        dcterms:coverage ;
    skos:definition "الخصائص المكانية للموارد: الخصائص التي تصف موقع الموارد وتوزيعها وحجمها وأبعادها في الفضاء الجغرافي."@arabic ;
    skos:prefLabel "التغطية المكانية"@arabic .

dcterms:subject a rdf:Property ;
    rdfs:label "Subject"@en ;
    dcterms:description "Recommended practice is to refer to the subject with a URI. If this is not possible or feasible, a literal value that identifies the subject may be provided. Both should preferably refer to a subject in a controlled vocabulary."@en ;
    dcterms:issued "2008-01-14"^^xsd:date ;
    rdfs:comment "A topic of the resource."@en ;
    rdfs:isDefinedBy dcterms: ;
    rdfs:subPropertyOf dc:subject ;
    skos:definition "الموضوع المرتبط بالمورد أو الموضوع الذي يتناوله المورد."@arabic ;
    skos:prefLabel "الموضوع"@arabic .

dcterms:tableOfContents a rdf:Property ;
    rdfs:label "Table Of Contents"@en ;
    dcterms:issued "2000-07-11"^^xsd:date ;
    rdfs:comment "A list of subunits of the resource."@en ;
    rdfs:isDefinedBy dcterms: ;
    rdfs:subPropertyOf dc:description,
        dcterms:description ;
    skos:definition "قائمة بالوحدات الفرعية للموارد."@arabic ;
    skos:prefLabel "جدول المحتويات"@arabic .

dcterms:temporal a rdf:Property ;
    rdfs:label "Temporal Coverage"@en ;
    dcam:rangeIncludes dcterms:PeriodOfTime ;
    dcterms:issued "2000-07-11"^^xsd:date ;
    rdfs:comment "Temporal characteristics of the resource."@en ;
    rdfs:isDefinedBy dcterms: ;
    rdfs:subPropertyOf dc:coverage,
        dcterms:coverage ;
    skos:definition "الخصائص الزمنية للموارد: تشير إلى توقيت ومواقيت ومعدلات وتكرار وأطوال المدة والتتابع الزمني المرتبط باستخدام أو توافر المورد."@arabic ;
    skos:prefLabel "التغطية الزمنية"@arabic .

dcterms:type a rdf:Property ;
    rdfs:label "Type"@en ;
    dcterms:description "Recommended practice is to use a controlled vocabulary such as the DCMI Type Vocabulary [[DCMI-TYPE](http://dublincore.org/documents/dcmi-type-vocabulary/)]. To describe the file format, physical medium, or dimensions of the resource, use the property Format."@en ;
    dcterms:issued "2008-01-14"^^xsd:date ;
    rdfs:comment "The nature or genre of the resource."@en ;
    rdfs:isDefinedBy dcterms: ;
    rdfs:subPropertyOf dc:type ;
    skos:definition "النوع أو الفئة التي ينتمي إليها المورد."@arabic ;
    skos:prefLabel "النوع"@arabic .

dcterms:valid a rdf:Property ;
    rdfs:label "Date Valid"@en ;
    dcterms:description "Recommended practice is to describe the date, date/time, or period of time as recommended for the property Date, of which this is a subproperty."@en ;
    dcterms:issued "2000-07-11"^^xsd:date ;
    rdfs:comment "Date (often a range) of validity of a resource."@en ;
    rdfs:isDefinedBy dcterms: ;
    rdfs:range rdfs:Literal ;
    rdfs:subPropertyOf dc:date,
        dcterms:date ;
    skos:definition "التاريخ (أو نطاق التواريخ) الذي يحدد فترة صلاحية المورد."@arabic ;
    skos:prefLabel "التاريخ صالح"@arabic .

dcterms:Period a rdfs:Datatype ;
    rdfs:label "DCMI Period"@en ;
    dcterms:issued "2000-07-11"^^xsd:date ;
    rdfs:comment "The set of time intervals defined by their limits according to the DCMI Period Encoding Scheme."@en ;
    rdfs:isDefinedBy dcterms: ;
    rdfs:seeAlso <https://www.dublincore.org/specifications/dublin-core/dcmi-period/> .

dcterms:contributor a rdf:Property ;
    rdfs:label "Contributor"@en ;
    dcam:rangeIncludes dcterms:Agent ;
    dcterms:description "The guidelines for using names of persons or organizations as creators apply to contributors."@en ;
    dcterms:issued "2008-01-14"^^xsd:date ;
    rdfs:comment "An entity responsible for making contributions to the resource."@en ;
    rdfs:isDefinedBy dcterms: ;
    rdfs:subPropertyOf dc:contributor ;
    skos:definition "الجهة التي تقوم بتقديم إسهامات للموارد."@arabic ;
    skos:prefLabel "مساهم"@arabic .

dcterms:identifier a rdf:Property ;
    rdfs:label "Identifier"@en ;
    dcterms:description "Recommended practice is to identify the resource by means of a string conforming to an identification system. Examples include International Standard Book Number (ISBN), Digital Object Identifier (DOI), and Uniform Resource Name (URN).  Persistent identifiers should be provided as HTTP URIs."@en ;
    dcterms:issued "2008-01-14"^^xsd:date ;
    rdfs:comment "An unambiguous reference to the resource within a given context."@en ;
    rdfs:isDefinedBy dcterms: ;
    rdfs:range rdfs:Literal ;
    rdfs:subPropertyOf dc:identifier ;
    skos:definition "مرجع واضح ولا يحمل أي غموض للموارد داخل سياق محدد."@arabic ;
    skos:prefLabel "معرف"@arabic .

dcterms:title a rdf:Property ;
    rdfs:label "Title"@en ;
    dcterms:issued "2008-01-14"^^xsd:date ;
    rdfs:comment "A name given to the resource."@en ;
    rdfs:isDefinedBy dcterms: ;
    rdfs:range rdfs:Literal ;
    rdfs:subPropertyOf dc:title ;
    skos:definition "الاسم الذي يُمنح للموارد."@arabic ;
    skos:prefLabel "العنوان"@arabic .

dcterms:audience a rdf:Property ;
    rdfs:label "Audience"@en ;
    dcam:rangeIncludes dcterms:AgentClass ;
    dcterms:description "Recommended practice is to use this property with non-literal values from a vocabulary of audience types."@en ;
    dcterms:issued "2001-05-21"^^xsd:date ;
    rdfs:comment "A class of agents for whom the resource is intended or useful."@en ;
    rdfs:isDefinedBy dcterms: ;
    skos:definition "مجموعة من الوكلاء أو الكيانات التي يُقصد بها المورد أو التي تستفيد منه."@arabic ;
    skos:prefLabel "جمهور"@arabic .

dcterms:coverage a rdf:Property ;
    rdfs:label "Coverage"@en ;
    dcam:rangeIncludes dcterms:Jurisdiction,
        dcterms:Location,
        dcterms:Period ;
    dcterms:description "Spatial topic and spatial applicability may be a named place or a location specified by its geographic coordinates. Temporal topic may be a named period, date, or date range. A jurisdiction may be a named administrative entity or a geographic place to which the resource applies. Recommended practice is to use a controlled vocabulary such as the Getty Thesaurus of Geographic Names [[TGN](https://www.getty.edu/research/tools/vocabulary/tgn/index.html)]. Where appropriate, named places or time periods may be used in preference to numeric identifiers such as sets of coordinates or date ranges.  Because coverage is so broadly defined, it is preferable to use the more specific subproperties Temporal Coverage and Spatial Coverage."@en ;
    dcterms:issued "2008-01-14"^^xsd:date ;
    rdfs:comment "The spatial or temporal topic of the resource, spatial applicability of the resource, or jurisdiction under which the resource is relevant."@en ;
    rdfs:isDefinedBy dcterms: ;
    rdfs:subPropertyOf dc:coverage ;
    skos:definition "الموضوع المكاني أو الزمني للموارد، أو قابلية تطبيق الموقع للموارد، أو الولاية القضائية التي يقتضيها المورد."@arabic ;
    skos:prefLabel "التغطية"@arabic .

dcterms:description a rdf:Property ;
    rdfs:label "Description"@en ;
    dcterms:description "Description may include but is not limited to: an abstract, a table of contents, a graphical representation, or a free-text account of the resource."@en ;
    dcterms:issued "2008-01-14"^^xsd:date ;
    rdfs:comment "An account of the resource."@en ;
    rdfs:isDefinedBy dcterms: ;
    rdfs:subPropertyOf dc:description ;
    skos:definition "وصف أو توثيق للموارد."@arabic ;
    skos:prefLabel "الوصف"@arabic .

dcterms:format a rdf:Property ;
    rdfs:label "Format"@en ;
    dcam:rangeIncludes dcterms:Extent,
        dcterms:MediaType ;
    dcterms:description "Recommended practice is to use a controlled vocabulary where available. For example, for file formats one could use the list of Internet Media Types [[MIME](https://www.iana.org/assignments/media-types/media-types.xhtml)].  Examples of dimensions include size and duration."@en ;
    dcterms:issued "2008-01-14"^^xsd:date ;
    rdfs:comment "The file format, physical medium, or dimensions of the resource."@en ;
    rdfs:isDefinedBy dcterms: ;
    rdfs:subPropertyOf dc:format ;
    skos:definition "الملف أو الوسيط الفيزيائي أو الأبعاد المادية التي يحملها المورد."@arabic ;
    skos:prefLabel "التنسيق"@arabic .

dcterms:rights a rdf:Property ;
    rdfs:label "Rights"@en ;
    dcam:rangeIncludes dcterms:RightsStatement ;
    dcterms:description "Typically, rights information includes a statement about various property rights associated with the resource, including intellectual property rights.  Recommended practice is to refer to a rights statement with a URI.  If this is not possible or feasible, a literal value (name, label, or short text) may be provided."@en ;
    dcterms:issued "2008-01-14"^^xsd:date ;
    rdfs:comment "Information about rights held in and over the resource."@en ;
    rdfs:isDefinedBy dcterms: ;
    rdfs:subPropertyOf dc:rights ;
    skos:definition "معلومات عن الحقوق المملوكة للموارد والحقوق التي تُدار عليها."@arabic ;
    skos:prefLabel "الحقوق"@arabic .

dcterms:date a rdf:Property ;
    rdfs:label "Date"@en ;
    dcterms:description "Date may be used to express temporal information at any level of granularity.  Recommended practice is to express the date, date/time, or period of time according to ISO 8601-1 [[ISO 8601-1](https://www.iso.org/iso-8601-date-and-time-format.html)] or a published profile of the ISO standard, such as the W3C Note on Date and Time Formats [[W3CDTF](https://www.w3.org/TR/NOTE-datetime)] or the Extended Date/Time Format Specification [[EDTF](http://www.loc.gov/standards/datetime/)].  If the full date is unknown, month and year (YYYY-MM) or just year (YYYY) may be used. Date ranges may be specified using ISO 8601 period of time specification in which start and end dates are separated by a '/' (slash) character.  Either the start or end date may be missing."@en ;
    dcterms:issued "2008-01-14"^^xsd:date ;
    rdfs:comment "A point or period of time associated with an event in the lifecycle of the resource."@en ;
    rdfs:isDefinedBy dcterms: ;
    rdfs:range rdfs:Literal ;
    rdfs:subPropertyOf dc:date ;
    skos:definition "نقطة زمنية أو فترة زمنية مرتبطة بحدث في دورة حياة المورد."@arabic ;
    skos:prefLabel "التاريخ"@arabic .

dcterms:relation a rdf:Property ;
    rdfs:label "Relation"@en ;
    dcterms:description "Recommended practice is to identify the related resource by means of a URI.  If this is not possible or feasible, a string conforming to a formal identification system may be provided."@en ;
    dcterms:issued "2008-01-14"^^xsd:date ;
    rdfs:comment "A related resource."@en ;
    rdfs:isDefinedBy dcterms: ;
    rdfs:subPropertyOf dc:relation ;
    skos:definition "مصدر ذو صلة: مصدر مرتبط بمحتوى أو موضوع آخر، يشتمل على معلومات تتعلق أو تتقاطع مع الموضوع الأساسي."@arabic ;
    skos:prefLabel "علاقة"@arabic .

dcterms: dcterms:modified "2012-06-14"^^xsd:date ;
    dcterms:publisher <http://purl.org/dc/aboutdcmi#DCMI> ;
    dcterms:title "DCMI Metadata Terms - other"@en .

