@prefix dc: <http://purl.org/dc/elements/1.1/> .
@prefix dcam: <http://purl.org/dc/dcam/> .
@prefix dcmitype: <http://purl.org/dc/dcmitype/> .
@prefix dcterms: <http://purl.org/dc/terms/> .
@prefix foaf: <http://xmlns.com/foaf/0.1/> .
@prefix owl: <http://www.w3.org/2002/07/owl#> .
@prefix rdf: <http://www.w3.org/1999/02/22-rdf-syntax-ns#> .
@prefix rdfs: <http://www.w3.org/2000/01/rdf-schema#> .
@prefix skos: <http://www.w3.org/2004/02/skos/core#> .
@prefix xsd: <http://www.w3.org/2001/XMLSchema#> .

dcterms:Agent a dcterms:AgentClass,
        rdfs:Class ;
    rdfs:label "Agent"@en ;
    dcterms:issued "2008-01-14"^^xsd:date ;
    rdfs:comment "A resource that acts or has the power to act."@en ;
    rdfs:isDefinedBy dcterms: ;
    skos:definition "Un recurso que actúa o que tiene el poder de actuar."@es ;
    skos:prefLabel "Agente"@es .

dcterms:AgentClass a rdfs:Class ;
    rdfs:label "Agent Class"@en ;
    dcterms:issued "2008-01-14"^^xsd:date ;
    rdfs:comment "A group of agents."@en ;
    rdfs:isDefinedBy dcterms: ;
    rdfs:subClassOf rdfs:Class ;
    skos:definition "Un conjunto de agentes."@es ;
    skos:prefLabel "Clase de Agente"@es .

dcterms:BibliographicResource a rdfs:Class ;
    rdfs:label "Bibliographic Resource"@en ;
    dcterms:issued "2008-01-14"^^xsd:date ;
    rdfs:comment "A book, article, or other documentary resource."@en ;
    rdfs:isDefinedBy dcterms: ;
    skos:definition "Un libro, artículo u otro recurso documental."@es ;
    skos:prefLabel "Recurso Bibliográfico"@es .

dcterms:FileFormat a rdfs:Class ;
    rdfs:label "File Format"@en ;
    dcterms:issued "2008-01-14"^^xsd:date ;
    rdfs:comment "A digital resource format."@en ;
    rdfs:isDefinedBy dcterms: ;
    rdfs:subClassOf dcterms:MediaType ;
    skos:definition "Un formato de recurso digital es un estándar o estructura utilizada para almacenar, representar y facilitar el acceso a recursos digitales, como archivos, bases de datos o contenidos multimedia."@es ;
    skos:prefLabel "Formato de archivo"@es .

dcterms:Frequency a rdfs:Class ;
    rdfs:label "Frequency"@en ;
    dcterms:issued "2008-01-14"^^xsd:date ;
    rdfs:comment "A rate at which something recurs."@en ;
    rdfs:isDefinedBy dcterms: ;
    skos:definition "La frecuencia con la que algo se repite."@es ;
    skos:prefLabel "Frecuencia"@es .

dcterms:Jurisdiction a rdfs:Class ;
    rdfs:label "Jurisdiction"@en ;
    dcterms:issued "2008-01-14"^^xsd:date ;
    rdfs:comment "The extent or range of judicial, law enforcement, or other authority."@en ;
    rdfs:isDefinedBy dcterms: ;
    rdfs:subClassOf dcterms:LocationPeriodOrJurisdiction ;
    skos:definition "El alcance o extensión de la autoridad judicial, policial o de otro tipo."@es ;
    skos:prefLabel "Jurisdicción"@es .

dcterms:LicenseDocument a rdfs:Class ;
    rdfs:label "License Document"@en ;
    dcterms:issued "2008-01-14"^^xsd:date ;
    rdfs:comment "A legal document giving official permission to do something with a resource."@en ;
    rdfs:isDefinedBy dcterms: ;
    rdfs:subClassOf dcterms:RightsStatement ;
    skos:definition "Documento legal que concede permiso oficial para realizar alguna acción con un recurso."@es ;
    skos:prefLabel "Documento de Licencia"@es .

dcterms:LinguisticSystem a rdfs:Class ;
    rdfs:label "Linguistic System"@en ;
    dcterms:description "Written, spoken, sign, and computer languages are linguistic systems."@en ;
    dcterms:issued "2008-01-14"^^xsd:date ;
    rdfs:comment "A system of signs, symbols, sounds, gestures, or rules used in communication."@en ;
    rdfs:isDefinedBy dcterms: ;
    skos:definition "Un sistema de signos, símbolos, sonidos, gestos o reglas que se utilizan en la comunicación."@es ;
    skos:prefLabel "Sistema lingüístico"@es .

dcterms:Location a rdfs:Class ;
    rdfs:label "Location"@en ;
    dcterms:issued "2008-01-14"^^xsd:date ;
    rdfs:comment "A spatial region or named place."@en ;
    rdfs:isDefinedBy dcterms: ;
    rdfs:subClassOf dcterms:LocationPeriodOrJurisdiction ;
    skos:definition "Una zona espacial o lugar con nombre."@es ;
    skos:prefLabel "Ubicación"@es .

dcterms:LocationPeriodOrJurisdiction a rdfs:Class ;
    rdfs:label "Location, Period, or Jurisdiction"@en ;
    dcterms:issued "2008-01-14"^^xsd:date ;
    rdfs:comment "A location, period of time, or jurisdiction."@en ;
    rdfs:isDefinedBy dcterms: ;
    skos:definition "Un lugar, un periodo de tiempo o una jurisdicción."@es ;
    skos:prefLabel "Ubicación, período o jurisdicción"@es .

dcterms:MediaType a rdfs:Class ;
    rdfs:label "Media Type"@en ;
    dcterms:issued "2008-01-14"^^xsd:date ;
    rdfs:comment "A file format or physical medium."@en ;
    rdfs:isDefinedBy dcterms: ;
    rdfs:subClassOf dcterms:MediaTypeOrExtent ;
    skos:definition "Formato de archivo o medio físico."@es ;
    skos:prefLabel "Tipo de medio"@es .

dcterms:MediaTypeOrExtent a rdfs:Class ;
    rdfs:label "Media Type or Extent"@en ;
    dcterms:issued "2008-01-14"^^xsd:date ;
    rdfs:comment "A media type or extent."@en ;
    rdfs:isDefinedBy dcterms: ;
    skos:definition "Tipo de medio o extensión."@es ;
    skos:prefLabel "Tipo de medio o extensión"@es .

dcterms:MethodOfAccrual a rdfs:Class ;
    rdfs:label "Method of Accrual"@en ;
    dcterms:issued "2008-01-14"^^xsd:date ;
    rdfs:comment "A method by which resources are added to a collection."@en ;
    rdfs:isDefinedBy dcterms: ;
    skos:definition "Conjunto de procedimientos o técnicas que permiten añadir recursos a una colección."@es ;
    skos:prefLabel "Método de devengo"@es .

dcterms:MethodOfInstruction a rdfs:Class ;
    rdfs:label "Method of Instruction"@en ;
    dcterms:issued "2008-01-14"^^xsd:date ;
    rdfs:comment "A process that is used to engender knowledge, attitudes, and skills."@en ;
    rdfs:isDefinedBy dcterms: ;
    skos:definition "Un proceso destinado a generar conocimiento, actitudes y habilidades."@es ;
    skos:prefLabel "Método de Instrucción"@es .

dcterms:PeriodOfTime a rdfs:Class ;
    rdfs:label "Period of Time"@en ;
    dcterms:issued "2008-01-14"^^xsd:date ;
    rdfs:comment "An interval of time that is named or defined by its start and end dates."@en ;
    rdfs:isDefinedBy dcterms: ;
    rdfs:subClassOf dcterms:LocationPeriodOrJurisdiction ;
    skos:definition "Un intervalo de tiempo que se nombra o define por sus fechas de inicio y fin."@es ;
    skos:prefLabel "Período de tiempo"@es .

dcterms:PhysicalMedium a rdfs:Class ;
    rdfs:label "Physical Medium"@en ;
    dcterms:description "Examples include paper, canvas, or DVD."@en ;
    dcterms:issued "2008-01-14"^^xsd:date ;
    rdfs:comment "A physical material or carrier."@en ;
    rdfs:isDefinedBy dcterms: ;
    rdfs:subClassOf dcterms:MediaType ;
    skos:definition "Material físico o soporte."@es ;
    skos:prefLabel "Medio físico"@es .

dcterms:PhysicalResource a rdfs:Class ;
    rdfs:label "Physical Resource"@en ;
    dcterms:issued "2008-01-14"^^xsd:date ;
    rdfs:comment "A material thing."@en ;
    rdfs:isDefinedBy dcterms: ;
    skos:definition "Un objeto con existencia física."@es ;
    skos:prefLabel "Recurso físico"@es .

dcterms:Policy a rdfs:Class ;
    rdfs:label "Policy"@en ;
    dcterms:issued "2008-01-14"^^xsd:date ;
    rdfs:comment "A plan or course of action by an authority, intended to influence and determine decisions, actions, and other matters."@en ;
    rdfs:isDefinedBy dcterms: ;
    skos:definition "Un plan o curso de acción elaborado por una autoridad con el propósito de influir y determinar decisiones, acciones y otros asuntos."@es ;
    skos:prefLabel "Política"@es .

dcterms:ProvenanceStatement a rdfs:Class ;
    rdfs:label "Provenance Statement"@en ;
    dcterms:issued "2008-01-14"^^xsd:date ;
    rdfs:comment "Any changes in ownership and custody of a resource since its creation that are significant for its authenticity, integrity, and interpretation."@en ;
    rdfs:isDefinedBy dcterms: ;
    skos:definition "Cualquier cambio en la propiedad y custodia de un recurso desde su creación que sea relevante para su autenticidad, integridad e interpretación."@es ;
    skos:prefLabel "Declaración de procedencia"@es .

dcterms:RightsStatement a rdfs:Class ;
    rdfs:label "Rights Statement"@en ;
    dcterms:issued "2008-01-14"^^xsd:date ;
    rdfs:comment "A statement about the intellectual property rights (IPR) held in or over a resource, a legal document giving official permission to do something with a resource, or a statement about access rights."@en ;
    rdfs:isDefinedBy dcterms: ;
    skos:definition "Una declaración acerca de los derechos de propiedad intelectual (IPR) que se poseen sobre un recurso, un documento legal que otorga permiso oficial para realizar alguna acción con dicho recurso, o una declaración sobre derechos de acceso."@es ;
    skos:prefLabel "Declaración de derechos"@es .

dcterms:SizeOrDuration a rdfs:Class ;
    rdfs:label "Size or Duration"@en ;
    dcterms:description "Examples include a number of pages, a specification of length, width, and breadth, or a period in hours, minutes, and seconds."@en ;
    dcterms:issued "2008-01-14"^^xsd:date ;
    rdfs:comment "A dimension or extent, or a time taken to play or execute."@en ;
    rdfs:isDefinedBy dcterms: ;
    rdfs:subClassOf dcterms:MediaTypeOrExtent ;
    skos:definition "Una dimensión o extensión, o el tiempo que se tarda en reproducir o ejecutar."@es ;
    skos:prefLabel "Tamaño o Duración"@es .

dcterms:Standard a rdfs:Class ;
    rdfs:label "Standard"@en ;
    dcterms:issued "2008-01-14"^^xsd:date ;
    rdfs:comment "A reference point against which other things can be evaluated or compared."@en ;
    rdfs:isDefinedBy dcterms: ;
    skos:definition "Punto de referencia contra el cual se pueden evaluar o comparar otras cosas."@es ;
    skos:prefLabel "Estándar"@es .

dcterms:Box a rdfs:Datatype ;
    rdfs:label "DCMI Box"@en ;
    dcterms:issued "2000-07-11"^^xsd:date ;
    rdfs:comment "The set of regions in space defined by their geographic coordinates according to the DCMI Box Encoding Scheme."@en ;
    rdfs:isDefinedBy dcterms: ;
    rdfs:seeAlso <https://www.dublincore.org/specifications/dublin-core/dcmi-box/> .

dcterms:DCMIType a dcam:VocabularyEncodingScheme ;
    rdfs:label "DCMI Type Vocabulary"@en ;
    dcterms:issued "2000-07-11"^^xsd:date ;
    rdfs:comment "The set of classes specified by the DCMI Type Vocabulary, used to categorize the nature or genre of the resource."@en ;
    rdfs:isDefinedBy dcterms: ;
    rdfs:seeAlso dcmitype: .

dcterms:DDC a dcam:VocabularyEncodingScheme ;
    rdfs:label "DDC"@en ;
    dcterms:issued "2000-07-11"^^xsd:date ;
    rdfs:comment "The set of conceptual resources specified by the Dewey Decimal Classification."@en ;
    rdfs:isDefinedBy dcterms: ;
    rdfs:seeAlso <http://www.oclc.org/dewey/> .

dcterms:IMT a dcam:VocabularyEncodingScheme ;
    rdfs:label "IMT"@en ;
    dcterms:issued "2000-07-11"^^xsd:date ;
    rdfs:comment "The set of media types specified by the Internet Assigned Numbers Authority."@en ;
    rdfs:isDefinedBy dcterms: ;
    rdfs:seeAlso <http://www.iana.org/assignments/media-types/> .

dcterms:ISO3166 a rdfs:Datatype ;
    rdfs:label "ISO 3166"@en ;
    dcterms:issued "2000-07-11"^^xsd:date ;
    rdfs:comment "The set of codes listed in ISO 3166-1 for the representation of names of countries."@en ;
    rdfs:isDefinedBy dcterms: ;
    rdfs:seeAlso <https://www.iso.org/obp/ui/#search> .

dcterms:ISO639-2 a rdfs:Datatype ;
    rdfs:label "ISO 639-2"@en ;
    dcterms:issued "2000-07-11"^^xsd:date ;
    rdfs:comment "The three-letter alphabetic codes listed in ISO639-2 for the representation of names of languages."@en ;
    rdfs:isDefinedBy dcterms: ;
    rdfs:seeAlso <http://lcweb.loc.gov/standards/iso639-2/langhome.html> .

dcterms:ISO639-3 a rdfs:Datatype ;
    rdfs:label "ISO 639-3"@en ;
    dcterms:issued "2008-01-14"^^xsd:date ;
    rdfs:comment "The set of three-letter codes listed in ISO 639-3 for the representation of names of languages."@en ;
    rdfs:isDefinedBy dcterms: ;
    rdfs:seeAlso <http://www.sil.org/iso639-3/> .

dcterms:LCC a dcam:VocabularyEncodingScheme ;
    rdfs:label "LCC"@en ;
    dcterms:issued "2000-07-11"^^xsd:date ;
    rdfs:comment "The set of conceptual resources specified by the Library of Congress Classification."@en ;
    rdfs:isDefinedBy dcterms: ;
    rdfs:seeAlso <http://lcweb.loc.gov/catdir/cpso/lcco/lcco.html> .

dcterms:LCSH a dcam:VocabularyEncodingScheme ;
    rdfs:label "LCSH"@en ;
    dcterms:issued "2000-07-11"^^xsd:date ;
    rdfs:comment "The set of labeled concepts specified by the Library of Congress Subject Headings."@en ;
    rdfs:isDefinedBy dcterms: .

dcterms:MESH a dcam:VocabularyEncodingScheme ;
    rdfs:label "MeSH"@en ;
    dcterms:issued "2000-07-11"^^xsd:date ;
    rdfs:comment "The set of labeled concepts specified by the Medical Subject Headings."@en ;
    rdfs:isDefinedBy dcterms: ;
    rdfs:seeAlso <http://www.nlm.nih.gov/mesh/meshhome.html> .

dcterms:NLM a dcam:VocabularyEncodingScheme ;
    rdfs:label "NLM"@en ;
    dcterms:issued "2005-06-13"^^xsd:date ;
    rdfs:comment "The set of conceptual resources specified by the National Library of Medicine Classification."@en ;
    rdfs:isDefinedBy dcterms: ;
    rdfs:seeAlso <http://wwwcf.nlm.nih.gov/class/> .

dcterms:Point a rdfs:Datatype ;
    rdfs:label "DCMI Point"@en ;
    dcterms:issued "2000-07-11"^^xsd:date ;
    rdfs:comment "The set of points in space defined by their geographic coordinates according to the DCMI Point Encoding Scheme."@en ;
    rdfs:isDefinedBy dcterms: ;
    rdfs:seeAlso <https://www.dublincore.org/specifications/dublin-core/dcmi-point/> .

dcterms:RFC1766 a rdfs:Datatype ;
    rdfs:label "RFC 1766"@en ;
    dcterms:issued "2000-07-11"^^xsd:date ;
    rdfs:comment "The set of tags, constructed according to RFC 1766, for the identification of languages."@en ;
    rdfs:isDefinedBy dcterms: ;
    rdfs:seeAlso <http://www.ietf.org/rfc/rfc1766.txt> .

dcterms:RFC3066 a rdfs:Datatype ;
    rdfs:label "RFC 3066"@en ;
    dcterms:description "RFC 3066 has been obsoleted by RFC 4646."@en ;
    dcterms:issued "2002-07-13"^^xsd:date ;
    rdfs:comment "The set of tags constructed according to RFC 3066 for the identification of languages."@en ;
    rdfs:isDefinedBy dcterms: ;
    rdfs:seeAlso <http://www.ietf.org/rfc/rfc3066.txt> .

dcterms:RFC4646 a rdfs:Datatype ;
    rdfs:label "RFC 4646"@en ;
    dcterms:description "RFC 4646 obsoletes RFC 3066."@en ;
    dcterms:issued "2008-01-14"^^xsd:date ;
    rdfs:comment "The set of tags constructed according to RFC 4646 for the identification of languages."@en ;
    rdfs:isDefinedBy dcterms: ;
    rdfs:seeAlso <http://www.ietf.org/rfc/rfc4646.txt> .

dcterms:RFC5646 a rdfs:Datatype ;
    rdfs:label "RFC 5646"@en ;
    dcterms:description "RFC 5646 obsoletes RFC 4646."@en ;
    dcterms:issued "2010-10-11"^^xsd:date ;
    rdfs:comment "The set of tags constructed according to RFC 5646 for the identification of languages."@en ;
    rdfs:isDefinedBy dcterms: ;
    rdfs:seeAlso <http://www.ietf.org/rfc/rfc5646.txt> .

dcterms:TGN a dcam:VocabularyEncodingScheme ;
    rdfs:label "TGN"@en ;
    dcterms:issued "2000-07-11"^^xsd:date ;
    rdfs:comment "The set of places specified by the Getty Thesaurus of Geographic Names."@en ;
    rdfs:isDefinedBy dcterms: ;
    rdfs:seeAlso <http://www.getty.edu/research/tools/vocabulary/tgn/index.html> .

dcterms:UDC a dcam:VocabularyEncodingScheme ;
    rdfs:label "UDC"@en ;
    dcterms:issued "2000-07-11"^^xsd:date ;
    rdfs:comment "The set of conceptual resources specified by the Universal Decimal Classification."@en ;
    rdfs:isDefinedBy dcterms: ;
    rdfs:seeAlso <http://www.udcc.org/> .

dcterms:URI a rdfs:Datatype ;
    rdfs:label "URI"@en ;
    dcterms:issued "2000-07-11"^^xsd:date ;
    rdfs:comment "The set of identifiers constructed according to the generic syntax for Uniform Resource Identifiers as specified by the Internet Engineering Task Force."@en ;
    rdfs:isDefinedBy dcterms: ;
    rdfs:seeAlso <http://www.ietf.org/rfc/rfc3986.txt> .

dcterms:W3CDTF a rdfs:Datatype ;
    rdfs:label "W3C-DTF"@en ;
    dcterms:issued "2000-07-11"^^xsd:date ;
    rdfs:comment "The set of dates and times constructed according to the W3C Date and Time Formats Specification."@en ;
    rdfs:isDefinedBy dcterms: ;
    rdfs:seeAlso <http://www.w3.org/TR/NOTE-datetime> .

dcterms:abstract a rdf:Property ;
    rdfs:label "Abstract"@en ;
    dcterms:issued "2000-07-11"^^xsd:date ;
    rdfs:comment "A summary of the resource."@en ;
    rdfs:isDefinedBy dcterms: ;
    rdfs:subPropertyOf dc:description,
        dcterms:description ;
    skos:definition "Un resumen del recurso."@es ;
    skos:prefLabel "Resumen"@es .

dcterms:accessRights a rdf:Property ;
    rdfs:label "Access Rights"@en ;
    dcam:rangeIncludes dcterms:RightsStatement ;
    dcterms:description "Access Rights may include information regarding access or restrictions based on privacy, security, or other policies."@en ;
    dcterms:issued "2003-02-15"^^xsd:date ;
    rdfs:comment "Information about who access the resource or an indication of its security status."@en ;
    rdfs:isDefinedBy dcterms: ;
    rdfs:subPropertyOf dc:rights,
        dcterms:rights ;
    skos:definition "Información sobre quién accede al recurso o indicación de su estado de seguridad."@es ;
    skos:prefLabel "Derechos de acceso"@es .

dcterms:accrualMethod a rdf:Property ;
    rdfs:label "Accrual Method"@en ;
    dcam:rangeIncludes dcterms:MethodOfAccrual ;
    dcterms:description "Recommended practice is to use a value from the Collection Description Accrual Method Vocabulary [[DCMI-ACCRUALMETHOD](https://dublincore.org/groups/collections/accrual-method/)]."@en ;
    dcterms:issued "2005-06-13"^^xsd:date ;
    rdfs:comment "The method by which items are added to a collection."@en ;
    rdfs:domain dcmitype:Collection ;
    rdfs:isDefinedBy dcterms: ;
    skos:definition "El proceso o técnica mediante el cual se añaden elementos a una colección."@es ;
    skos:prefLabel "Método de devengo"@es .

dcterms:accrualPeriodicity a rdf:Property ;
    rdfs:label "Accrual Periodicity"@en ;
    dcam:rangeIncludes dcterms:Frequency ;
    dcterms:description "Recommended practice is to use a value from the Collection Description Frequency Vocabulary [[DCMI-COLLFREQ](https://dublincore.org/groups/collections/frequency/)]."@en ;
    dcterms:issued "2005-06-13"^^xsd:date ;
    rdfs:comment "The frequency with which items are added to a collection."@en ;
    rdfs:domain dcmitype:Collection ;
    rdfs:isDefinedBy dcterms: ;
    skos:definition "La frecuencia con la que se añaden artículos a una colección."@es ;
    skos:prefLabel "Periodicidad de devengo"@es .

dcterms:accrualPolicy a rdf:Property ;
    rdfs:label "Accrual Policy"@en ;
    dcam:rangeIncludes dcterms:Policy ;
    dcterms:description "Recommended practice is to use a value from the Collection Description Accrual Policy Vocabulary [[DCMI-ACCRUALPOLICY](https://dublincore.org/groups/collections/accrual-policy/)]."@en ;
    dcterms:issued "2005-06-13"^^xsd:date ;
    rdfs:comment "The policy governing the addition of items to a collection."@en ;
    rdfs:domain dcmitype:Collection ;
    rdfs:isDefinedBy dcterms: ;
    skos:definition "Reglas y directrices que determinan cómo y bajo qué condiciones se añaden elementos a una colección."@es ;
    skos:prefLabel "Política de devengo"@es .

dcterms:alternative a rdf:Property ;
    rdfs:label "Alternative Title"@en ;
    dcterms:description "The distinction between titles and alternative titles is application-specific."@en ;
    dcterms:issued "2000-07-11"^^xsd:date ;
    rdfs:comment "An alternative name for the resource."@en ;
    rdfs:isDefinedBy dcterms: ;
    rdfs:range rdfs:Literal ;
    rdfs:subPropertyOf dc:title,
        dcterms:title ;
    skos:definition "Un nombre alternativo para el recurso."@es ;
    skos:prefLabel "Título alternativo"@es .

dcterms:available a rdf:Property ;
    rdfs:label "Date Available"@en ;
    dcterms:description "Recommended practice is to describe the date, date/time, or period of time as recommended for the property Date, of which this is a subproperty."@en ;
    dcterms:issued "2000-07-11"^^xsd:date ;
    rdfs:comment "Date that the resource became or will become available."@en ;
    rdfs:isDefinedBy dcterms: ;
    rdfs:range rdfs:Literal ;
    rdfs:subPropertyOf dc:date,
        dcterms:date ;
    skos:definition "Fecha en la que el recurso se hizo o hará disponible."@es ;
    skos:prefLabel "Fecha disponible"@es .

dcterms:bibliographicCitation a rdf:Property ;
    rdfs:label "Bibliographic Citation"@en ;
    dcterms:description "Recommended practice is to include sufficient bibliographic detail to identify the resource as unambiguously as possible."@en ;
    dcterms:issued "2003-02-15"^^xsd:date ;
    rdfs:comment "A bibliographic reference for the resource."@en ;
    rdfs:isDefinedBy dcterms: ;
    rdfs:range rdfs:Literal ;
    rdfs:subPropertyOf dc:identifier,
        dcterms:identifier ;
    skos:definition "Referencia bibliográfica del recurso: la descripción estandarizada que identifica y localiza un recurso, incluyendo datos como autor, título, editorial, año de publicación y demás información bibliográfica relevante."@es ;
    skos:prefLabel "Cita Bibliográfica"@es .

dcterms:conformsTo a rdf:Property ;
    rdfs:label "Conforms To"@en ;
    dcam:rangeIncludes dcterms:Standard ;
    dcterms:issued "2001-05-21"^^xsd:date ;
    rdfs:comment "An established standard to which the described resource conforms."@en ;
    rdfs:isDefinedBy dcterms: ;
    rdfs:subPropertyOf dc:relation,
        dcterms:relation ;
    skos:definition "Un estándar establecido al que el recurso descrito se ajusta."@es ;
    skos:prefLabel "Cumple con"@es .

dcterms:created a rdf:Property ;
    rdfs:label "Date Created"@en ;
    dcterms:description "Recommended practice is to describe the date, date/time, or period of time as recommended for the property Date, of which this is a subproperty."@en ;
    dcterms:issued "2000-07-11"^^xsd:date ;
    rdfs:comment "Date of creation of the resource."@en ;
    rdfs:isDefinedBy dcterms: ;
    rdfs:range rdfs:Literal ;
    rdfs:subPropertyOf dc:date,
        dcterms:date ;
    skos:definition "Fecha de creación del recurso."@es ;
    skos:prefLabel "Fecha de creación"@es .

dcterms:creator a rdf:Property ;
    rdfs:label "Creator"@en ;
    dcam:rangeIncludes dcterms:Agent ;
    dcterms:description "Recommended practice is to identify the creator with a URI.  If this is not possible or feasible, a literal value that identifies the creator may be provided."@en ;
    dcterms:issued "2008-01-14"^^xsd:date ;
    rdfs:comment "An entity responsible for making the resource."@en ;
    rdfs:isDefinedBy dcterms: ;
    rdfs:subPropertyOf dc:creator,
        dcterms:contributor ;
    owl:equivalentProperty foaf:maker ;
    skos:definition "Entidad encargada de crear el recurso."@es ;
    skos:prefLabel "Creador"@es .

dcterms:dateAccepted a rdf:Property ;
    rdfs:label "Date Accepted"@en ;
    dcterms:description "Recommended practice is to describe the date, date/time, or period of time as recommended for the property Date, of which this is a subproperty.  Examples of resources to which a date of acceptance may be relevant are a thesis (accepted by a university department) or an article (accepted by a journal)."@en ;
    dcterms:issued "2002-07-13"^^xsd:date ;
    rdfs:comment "Date of acceptance of the resource."@en ;
    rdfs:isDefinedBy dcterms: ;
    rdfs:range rdfs:Literal ;
    rdfs:subPropertyOf dc:date,
        dcterms:date ;
    skos:definition "Fecha en que se aceptó el recurso."@es ;
    skos:prefLabel "Fecha de aceptación"@es .

dcterms:dateCopyrighted a rdf:Property ;
    rdfs:label "Date Copyrighted"@en ;
    dcterms:description "Typically a year.  Recommended practice is to describe the date, date/time, or period of time as recommended for the property Date, of which this is a subproperty."@en ;
    dcterms:issued "2002-07-13"^^xsd:date ;
    rdfs:comment "Date of copyright of the resource."@en ;
    rdfs:isDefinedBy dcterms: ;
    rdfs:range rdfs:Literal ;
    rdfs:subPropertyOf dc:date,
        dcterms:date ;
    skos:definition "Fecha en que se registró el derecho de autor del recurso."@es ;
    skos:prefLabel "Fecha de derechos de autor"@es .

dcterms:dateSubmitted a rdf:Property ;
    rdfs:label "Date Submitted"@en ;
    dcterms:description "Recommended practice is to describe the date, date/time, or period of time as recommended for the property Date, of which this is a subproperty.  Examples of resources to which a 'Date Submitted' may be relevant include a thesis (submitted to a university department) or an article (submitted to a journal)."@en ;
    dcterms:issued "2002-07-13"^^xsd:date ;
    rdfs:comment "Date of submission of the resource."@en ;
    rdfs:isDefinedBy dcterms: ;
    rdfs:range rdfs:Literal ;
    rdfs:subPropertyOf dc:date,
        dcterms:date ;
    skos:definition "Fecha de envío del recurso."@es ;
    skos:prefLabel "Fecha de envío"@es .

dcterms:educationLevel a rdf:Property ;
    rdfs:label "Audience Education Level"@en ;
    dcam:rangeIncludes dcterms:AgentClass ;
    dcterms:issued "2002-07-13"^^xsd:date ;
    rdfs:comment "A class of agents, defined in terms of progression through an educational or training context, for which the described resource is intended."@en ;
    rdfs:isDefinedBy dcterms: ;
    rdfs:subPropertyOf dcterms:audience ;
    skos:definition "Una categoría de agentes, definida por su progreso dentro de un contexto educativo o de capacitación, a quienes está destinado el recurso descrito."@es ;
    skos:prefLabel "Nivel educativo de la audiencia"@es .

dcterms:extent a rdf:Property ;
    rdfs:label "Extent"@en ;
    dcam:rangeIncludes dcterms:SizeOrDuration ;
    dcterms:description "Recommended practice is to specify the file size in megabytes and duration in ISO 8601 format."@en ;
    dcterms:issued "2000-07-11"^^xsd:date ;
    rdfs:comment "The size or duration of the resource."@en ;
    rdfs:isDefinedBy dcterms: ;
    rdfs:subPropertyOf dc:format,
        dcterms:format ;
    skos:definition "El tamaño o la duración de un recurso."@es ;
    skos:prefLabel "Extensión"@es .

dcterms:hasFormat a rdf:Property ;
    rdfs:label "Has Format"@en ;
    dcterms:description "This property is intended to be used with non-literal values. This property is an inverse property of Is Format Of."@en ;
    dcterms:issued "2000-07-11"^^xsd:date ;
    rdfs:comment "A related resource that is substantially the same as the pre-existing described resource, but in another format."@en ;
    rdfs:isDefinedBy dcterms: ;
    rdfs:subPropertyOf dc:relation,
        dcterms:relation ;
    skos:definition "Recurso relacionado que es sustancialmente equivalente al recurso descrito previamente, pero en un formato diferente."@es ;
    skos:prefLabel "Tiene formato"@es .

dcterms:hasPart a rdf:Property ;
    rdfs:label "Has Part"@en ;
    dcterms:description "This property is intended to be used with non-literal values. This property is an inverse property of Is Part Of."@en ;
    dcterms:issued "2000-07-11"^^xsd:date ;
    rdfs:comment "A related resource that is included either physically or logically in the described resource."@en ;
    rdfs:isDefinedBy dcterms: ;
    rdfs:subPropertyOf dc:relation,
        dcterms:relation ;
    skos:definition "Un recurso relacionado que se incluye, ya sea de forma física o lógica, en el recurso descrito."@es ;
    skos:prefLabel "Tiene parte"@es .

dcterms:hasVersion a rdf:Property ;
    rdfs:label "Has Version"@en ;
    dcterms:description "Changes in version imply substantive changes in content rather than differences in format. This property is intended to be used with non-literal values. This property is an inverse property of Is Version Of."@en ;
    dcterms:issued "2000-07-11"^^xsd:date ;
    rdfs:comment "A related resource that is a version, edition, or adaptation of the described resource."@en ;
    rdfs:isDefinedBy dcterms: ;
    rdfs:subPropertyOf dc:relation,
        dcterms:relation ;
    skos:definition "Un recurso relacionado que es una versión, edición o adaptación del recurso descrito."@es ;
    skos:prefLabel "Tiene Versión"@es .

dcterms:instructionalMethod a rdf:Property ;
    rdfs:label "Instructional Method"@en ;
    dcam:rangeIncludes dcterms:MethodOfInstruction ;
    dcterms:description "Instructional Method typically includes ways of presenting instructional materials or conducting instructional activities, patterns of learner-to-learner and learner-to-instructor interactions, and mechanisms by which group and individual levels of learning are measured.  Instructional methods include all aspects of the instruction and learning processes from planning and implementation through evaluation and feedback."@en ;
    dcterms:issued "2005-06-13"^^xsd:date ;
    rdfs:comment "A process, used to engender knowledge, attitudes and skills, that the described resource is designed to support."@en ;
    rdfs:isDefinedBy dcterms: ;
    skos:definition "Proceso utilizado para generar conocimiento, actitudes y habilidades, el cual el recurso descrito está diseñado para apoyar."@es ;
    skos:prefLabel "Método de instrucción"@es .

dcterms:isFormatOf a rdf:Property ;
    rdfs:label "Is Format Of"@en ;
    dcterms:description "This property is intended to be used with non-literal values. This property is an inverse property of Has Format."@en ;
    dcterms:issued "2000-07-11"^^xsd:date ;
    rdfs:comment "A pre-existing related resource that is substantially the same as the described resource, but in another format."@en ;
    rdfs:isDefinedBy dcterms: ;
    rdfs:subPropertyOf dc:relation,
        dcterms:relation ;
    skos:definition "Un recurso preexistente relacionado que es sustancialmente idéntico al recurso descrito, pero en otro formato."@es ;
    skos:prefLabel "Es formato de"@es .

dcterms:isPartOf a rdf:Property ;
    rdfs:label "Is Part Of"@en ;
    dcterms:description "This property is intended to be used with non-literal values. This property is an inverse property of Has Part."@en ;
    dcterms:issued "2000-07-11"^^xsd:date ;
    rdfs:comment "A related resource in which the described resource is physically or logically included."@en ;
    rdfs:isDefinedBy dcterms: ;
    rdfs:subPropertyOf dc:relation,
        dcterms:relation ;
    skos:definition "Un recurso relacionado en el que el recurso descrito está incluido física o lógicamente."@es ;
    skos:prefLabel "Es parte de"@es .

dcterms:isReferencedBy a rdf:Property ;
    rdfs:label "Is Referenced By"@en ;
    dcterms:description "This property is intended to be used with non-literal values. This property is an inverse property of References."@en ;
    dcterms:issued "2000-07-11"^^xsd:date ;
    rdfs:comment "A related resource that references, cites, or otherwise points to the described resource."@en ;
    rdfs:isDefinedBy dcterms: ;
    rdfs:subPropertyOf dc:relation,
        dcterms:relation ;
    skos:definition "Un recurso relacionado que referencia, cita o señala de alguna manera al recurso descrito."@es ;
    skos:prefLabel "Referenciado por"@es .

dcterms:isReplacedBy a rdf:Property ;
    rdfs:label "Is Replaced By"@en ;
    dcterms:description "This property is intended to be used with non-literal values. This property is an inverse property of Replaces."@en ;
    dcterms:issued "2000-07-11"^^xsd:date ;
    rdfs:comment "A related resource that supplants, displaces, or supersedes the described resource."@en ;
    rdfs:isDefinedBy dcterms: ;
    rdfs:subPropertyOf dc:relation,
        dcterms:relation ;
    skos:definition "Un recurso relacionado que sustituye, desplaza o reemplaza al recurso descrito."@es ;
    skos:prefLabel "Es reemplazado por"@es .

dcterms:isRequiredBy a rdf:Property ;
    rdfs:label "Is Required By"@en ;
    dcterms:description "This property is intended to be used with non-literal values. This property is an inverse property of Requires."@en ;
    dcterms:issued "2000-07-11"^^xsd:date ;
    rdfs:comment "A related resource that requires the described resource to support its function, delivery, or coherence."@en ;
    rdfs:isDefinedBy dcterms: ;
    rdfs:subPropertyOf dc:relation,
        dcterms:relation ;
    skos:definition "Recurso relacionado que necesita el recurso descrito para apoyar su función, entrega o coherencia."@es ;
    skos:prefLabel "Requerido por"@es .

dcterms:isVersionOf a rdf:Property ;
    rdfs:label "Is Version Of"@en ;
    dcterms:description "Changes in version imply substantive changes in content rather than differences in format. This property is intended to be used with non-literal values. This property is an inverse property of Has Version."@en ;
    dcterms:issued "2000-07-11"^^xsd:date ;
    rdfs:comment "A related resource of which the described resource is a version, edition, or adaptation."@en ;
    rdfs:isDefinedBy dcterms: ;
    rdfs:subPropertyOf dc:relation,
        dcterms:relation ;
    skos:definition "Un recurso relacionado del cual el recurso descrito es una versión, edición o adaptación."@es ;
    skos:prefLabel "es versión de"@es .

dcterms:issued a rdf:Property ;
    rdfs:label "Date Issued"@en ;
    dcterms:description "Recommended practice is to describe the date, date/time, or period of time as recommended for the property Date, of which this is a subproperty."@en ;
    dcterms:issued "2000-07-11"^^xsd:date ;
    rdfs:comment "Date of formal issuance of the resource."@en ;
    rdfs:isDefinedBy dcterms: ;
    rdfs:range rdfs:Literal ;
    rdfs:subPropertyOf dc:date,
        dcterms:date ;
    skos:definition "Fecha en la que se emite formalmente el recurso."@es ;
    skos:prefLabel "Fecha de emisión"@es .

dcterms:language a rdf:Property ;
    rdfs:label "Language"@en ;
    dcam:rangeIncludes dcterms:LinguisticSystem ;
    dcterms:description "Recommended practice is to use either a non-literal value representing a language from a controlled vocabulary such as ISO 639-2 or ISO 639-3, or a literal value consisting of an IETF Best Current Practice 47 [[IETF-BCP47](https://tools.ietf.org/html/bcp47)] language tag."@en ;
    dcterms:issued "2008-01-14"^^xsd:date ;
    rdfs:comment "A language of the resource."@en ;
    rdfs:isDefinedBy dcterms: ;
    rdfs:subPropertyOf dc:language ;
    skos:definition "El lenguaje asociado al recurso."@es ;
    skos:prefLabel "Idioma"@es .

dcterms:license a rdf:Property ;
    rdfs:label "License"@en ;
    dcam:rangeIncludes dcterms:LicenseDocument ;
    dcterms:description "Recommended practice is to identify the license document with a URI. If this is not possible or feasible, a literal value that identifies the license may be provided."@en ;
    dcterms:issued "2004-06-14"^^xsd:date ;
    rdfs:comment "A legal document giving official permission to do something with the resource."@en ;
    rdfs:isDefinedBy dcterms: ;
    rdfs:subPropertyOf dc:rights,
        dcterms:rights ;
    skos:definition "Un documento legal que otorga permiso oficial para realizar una acción con el recurso."@es ;
    skos:prefLabel "Licencia"@es .

dcterms:mediator a rdf:Property ;
    rdfs:label "Mediator"@en ;
    dcam:rangeIncludes dcterms:AgentClass ;
    dcterms:description "In an educational context, a mediator might be a parent, teacher, teaching assistant, or care-giver."@en ;
    dcterms:issued "2001-05-21"^^xsd:date ;
    rdfs:comment "An entity that mediates access to the resource."@en ;
    rdfs:isDefinedBy dcterms: ;
    rdfs:subPropertyOf dcterms:audience ;
    skos:definition "Una entidad que intermedia el acceso a un recurso."@es ;
    skos:prefLabel "mediador"@es .

dcterms:medium a rdf:Property ;
    rdfs:label "Medium"@en ;
    dcam:domainIncludes dcterms:PhysicalResource ;
    dcam:rangeIncludes dcterms:PhysicalMedium ;
    dcterms:issued "2000-07-11"^^xsd:date ;
    rdfs:comment "The material or physical carrier of the resource."@en ;
    rdfs:isDefinedBy dcterms: ;
    rdfs:subPropertyOf dc:format,
        dcterms:format ;
    skos:definition "El medio material o físico que transporta o aloja el recurso."@es ;
    skos:prefLabel "Medio"@es .

dcterms:modified a rdf:Property ;
    rdfs:label "Date Modified"@en ;
    dcterms:description "Recommended practice is to describe the date, date/time, or period of time as recommended for the property Date, of which this is a subproperty."@en ;
    dcterms:issued "2000-07-11"^^xsd:date ;
    rdfs:comment "Date on which the resource was changed."@en ;
    rdfs:isDefinedBy dcterms: ;
    rdfs:range rdfs:Literal ;
    rdfs:subPropertyOf dc:date,
        dcterms:date ;
    skos:definition "Fecha en la que se modificó el recurso."@es ;
    skos:prefLabel "Fecha de modificación"@es .

dcterms:provenance a rdf:Property ;
    rdfs:label "Provenance"@en ;
    dcam:rangeIncludes dcterms:ProvenanceStatement ;
    dcterms:description "The statement may include a description of any changes successive custodians made to the resource."@en ;
    dcterms:issued "2004-09-20"^^xsd:date ;
    rdfs:comment "A statement of any changes in ownership and custody of the resource since its creation that are significant for its authenticity, integrity, and interpretation."@en ;
    rdfs:isDefinedBy dcterms: ;
    skos:definition "Declaración de cualquier cambio de propiedad y custodia del recurso desde su creación que sea significativo para su autenticidad, integridad e interpretación."@es ;
    skos:prefLabel "Procedencia"@es .

dcterms:publisher a rdf:Property ;
    rdfs:label "Publisher"@en ;
    dcam:rangeIncludes dcterms:Agent ;
    dcterms:issued "2008-01-14"^^xsd:date ;
    rdfs:comment "An entity responsible for making the resource available."@en ;
    rdfs:isDefinedBy dcterms: ;
    rdfs:subPropertyOf dc:publisher ;
    skos:definition "Entidad responsable de hacer que el recurso esté disponible."@es ;
    skos:prefLabel "Editor"@es .

dcterms:references a rdf:Property ;
    rdfs:label "References"@en ;
    dcterms:description "This property is intended to be used with non-literal values. This property is an inverse property of Is Referenced By."@en ;
    dcterms:issued "2000-07-11"^^xsd:date ;
    rdfs:comment "A related resource that is referenced, cited, or otherwise pointed to by the described resource."@en ;
    rdfs:isDefinedBy dcterms: ;
    rdfs:subPropertyOf dc:relation,
        dcterms:relation ;
    skos:definition "Un recurso relacionado que es referenciado, citado o de otro modo señalado por el recurso descrito."@es ;
    skos:prefLabel "Referencias"@es .

dcterms:replaces a rdf:Property ;
    rdfs:label "Replaces"@en ;
    dcterms:description "This property is intended to be used with non-literal values. This property is an inverse property of Is Replaced By."@en ;
    dcterms:issued "2000-07-11"^^xsd:date ;
    rdfs:comment "A related resource that is supplanted, displaced, or superseded by the described resource."@en ;
    rdfs:isDefinedBy dcterms: ;
    rdfs:subPropertyOf dc:relation,
        dcterms:relation ;
    skos:definition "Recurso relacionado que ha sido reemplazado, desplazado o sustituido por el recurso descrito."@es ;
    skos:prefLabel "Reemplaza"@es .

dcterms:requires a rdf:Property ;
    rdfs:label "Requires"@en ;
    dcterms:description "This property is intended to be used with non-literal values. This property is an inverse property of Is Required By."@en ;
    dcterms:issued "2000-07-11"^^xsd:date ;
    rdfs:comment "A related resource that is required by the described resource to support its function, delivery, or coherence."@en ;
    rdfs:isDefinedBy dcterms: ;
    rdfs:subPropertyOf dc:relation,
        dcterms:relation ;
    skos:definition "Recurso relacionado que es necesario por el recurso descrito para soportar su función, facilitar su entrega o mantener su coherencia."@es ;
    skos:prefLabel "Requiere"@es .

dcterms:rightsHolder a rdf:Property ;
    rdfs:label "Rights Holder"@en ;
    dcam:rangeIncludes dcterms:Agent ;
    dcterms:description "Recommended practice is to refer to the rights holder with a URI. If this is not possible or feasible, a literal value that identifies the rights holder may be provided."@en ;
    dcterms:issued "2004-06-14"^^xsd:date ;
    rdfs:comment "A person or organization owning or managing rights over the resource."@en ;
    rdfs:isDefinedBy dcterms: ;
    skos:definition "Persona u organización que posee o gestiona derechos sobre el recurso."@es ;
    skos:prefLabel "Titular de derechos"@es .

dcterms:source a rdf:Property ;
    rdfs:label "Source"@en ;
    dcterms:description "This property is intended to be used with non-literal values. The described resource may be derived from the related resource in whole or in part. Best practice is to identify the related resource by means of a URI or a string conforming to a formal identification system."@en ;
    dcterms:issued "2008-01-14"^^xsd:date ;
    rdfs:comment "A related resource from which the described resource is derived."@en ;
    rdfs:isDefinedBy dcterms: ;
    rdfs:subPropertyOf dc:source,
        dcterms:relation ;
    skos:definition "Un recurso relacionado del cual se deriva el recurso descrito."@es ;
    skos:prefLabel "Fuente"@es .

dcterms:spatial a rdf:Property ;
    rdfs:label "Spatial Coverage"@en ;
    dcam:rangeIncludes dcterms:Location ;
    dcterms:issued "2000-07-11"^^xsd:date ;
    rdfs:comment "Spatial characteristics of the resource."@en ;
    rdfs:isDefinedBy dcterms: ;
    rdfs:subPropertyOf dc:coverage,
        dcterms:coverage ;
    skos:definition "Características espaciales del recurso."@es ;
    skos:prefLabel "Cobertura espacial"@es .

dcterms:subject a rdf:Property ;
    rdfs:label "Subject"@en ;
    dcterms:description "Recommended practice is to refer to the subject with a URI. If this is not possible or feasible, a literal value that identifies the subject may be provided. Both should preferably refer to a subject in a controlled vocabulary."@en ;
    dcterms:issued "2008-01-14"^^xsd:date ;
    rdfs:comment "A topic of the resource."@en ;
    rdfs:isDefinedBy dcterms: ;
    rdfs:subPropertyOf dc:subject ;
    skos:definition "El tema que aborda el recurso."@es ;
    skos:prefLabel "Asunto"@es .

dcterms:tableOfContents a rdf:Property ;
    rdfs:label "Table Of Contents"@en ;
    dcterms:issued "2000-07-11"^^xsd:date ;
    rdfs:comment "A list of subunits of the resource."@en ;
    rdfs:isDefinedBy dcterms: ;
    rdfs:subPropertyOf dc:description,
        dcterms:description ;
    skos:definition "Una lista de subunidades del recurso."@es ;
    skos:prefLabel "Tabla de Contenidos"@es .

dcterms:temporal a rdf:Property ;
    rdfs:label "Temporal Coverage"@en ;
    dcam:rangeIncludes dcterms:PeriodOfTime ;
    dcterms:issued "2000-07-11"^^xsd:date ;
    rdfs:comment "Temporal characteristics of the resource."@en ;
    rdfs:isDefinedBy dcterms: ;
    rdfs:subPropertyOf dc:coverage,
        dcterms:coverage ;
    skos:definition "Propiedades que describen el comportamiento temporal de un recurso, incluyendo su disponibilidad, duración, frecuencia de acceso y los ciclos o intervalos en los que cambia su estado."@es ;
    skos:prefLabel "Cobertura temporal"@es .

dcterms:type a rdf:Property ;
    rdfs:label "Type"@en ;
    dcterms:description "Recommended practice is to use a controlled vocabulary such as the DCMI Type Vocabulary [[DCMI-TYPE](http://dublincore.org/documents/dcmi-type-vocabulary/)]. To describe the file format, physical medium, or dimensions of the resource, use the property Format."@en ;
    dcterms:issued "2008-01-14"^^xsd:date ;
    rdfs:comment "The nature or genre of the resource."@en ;
    rdfs:isDefinedBy dcterms: ;
    rdfs:subPropertyOf dc:type ;
    skos:definition "Tipo o categoría que describe la naturaleza o género del recurso."@es ;
    skos:prefLabel "Tipo"@es .

dcterms:valid a rdf:Property ;
    rdfs:label "Date Valid"@en ;
    dcterms:description "Recommended practice is to describe the date, date/time, or period of time as recommended for the property Date, of which this is a subproperty."@en ;
    dcterms:issued "2000-07-11"^^xsd:date ;
    rdfs:comment "Date (often a range) of validity of a resource."@en ;
    rdfs:isDefinedBy dcterms: ;
    rdfs:range rdfs:Literal ;
    rdfs:subPropertyOf dc:date,
        dcterms:date ;
    skos:definition "Fecha o rango de fechas que indica la validez de un recurso."@es ;
    skos:prefLabel "Fecha válida"@es .

dcterms:Period a rdfs:Datatype ;
    rdfs:label "DCMI Period"@en ;
    dcterms:issued "2000-07-11"^^xsd:date ;
    rdfs:comment "The set of time intervals defined by their limits according to the DCMI Period Encoding Scheme."@en ;
    rdfs:isDefinedBy dcterms: ;
    rdfs:seeAlso <https://www.dublincore.org/specifications/dublin-core/dcmi-period/> .

dcterms:contributor a rdf:Property ;
    rdfs:label "Contributor"@en ;
    dcam:rangeIncludes dcterms:Agent ;
    dcterms:description "The guidelines for using names of persons or organizations as creators apply to contributors."@en ;
    dcterms:issued "2008-01-14"^^xsd:date ;
    rdfs:comment "An entity responsible for making contributions to the resource."@en ;
    rdfs:isDefinedBy dcterms: ;
    rdfs:subPropertyOf dc:contributor ;
    skos:definition "Entidad responsable de aportar contribuciones al recurso."@es ;
    skos:prefLabel "Contribuyente"@es .

dcterms:identifier a rdf:Property ;
    rdfs:label "Identifier"@en ;
    dcterms:description "Recommended practice is to identify the resource by means of a string conforming to an identification system. Examples include International Standard Book Number (ISBN), Digital Object Identifier (DOI), and Uniform Resource Name (URN).  Persistent identifiers should be provided as HTTP URIs."@en ;
    dcterms:issued "2008-01-14"^^xsd:date ;
    rdfs:comment "An unambiguous reference to the resource within a given context."@en ;
    rdfs:isDefinedBy dcterms: ;
    rdfs:range rdfs:Literal ;
    rdfs:subPropertyOf dc:identifier ;
    skos:definition "Una referencia inequívoca al recurso dentro de un contexto dado."@es ;
    skos:prefLabel "Identificador"@es .

dcterms:title a rdf:Property ;
    rdfs:label "Title"@en ;
    dcterms:issued "2008-01-14"^^xsd:date ;
    rdfs:comment "A name given to the resource."@en ;
    rdfs:isDefinedBy dcterms: ;
    rdfs:range rdfs:Literal ;
    rdfs:subPropertyOf dc:title ;
    skos:definition "Un nombre asignado al recurso."@es ;
    skos:prefLabel "Título"@es .

dcterms:audience a rdf:Property ;
    rdfs:label "Audience"@en ;
    dcam:rangeIncludes dcterms:AgentClass ;
    dcterms:description "Recommended practice is to use this property with non-literal values from a vocabulary of audience types."@en ;
    dcterms:issued "2001-05-21"^^xsd:date ;
    rdfs:comment "A class of agents for whom the resource is intended or useful."@en ;
    rdfs:isDefinedBy dcterms: ;
    skos:definition "Una clase de agentes a los que el recurso está destinado o que pueden beneficiarse de él."@es ;
    skos:prefLabel "Audiencia"@es .

dcterms:coverage a rdf:Property ;
    rdfs:label "Coverage"@en ;
    dcam:rangeIncludes dcterms:Jurisdiction,
        dcterms:Location,
        dcterms:Period ;
    dcterms:description "Spatial topic and spatial applicability may be a named place or a location specified by its geographic coordinates. Temporal topic may be a named period, date, or date range. A jurisdiction may be a named administrative entity or a geographic place to which the resource applies. Recommended practice is to use a controlled vocabulary such as the Getty Thesaurus of Geographic Names [[TGN](https://www.getty.edu/research/tools/vocabulary/tgn/index.html)]. Where appropriate, named places or time periods may be used in preference to numeric identifiers such as sets of coordinates or date ranges.  Because coverage is so broadly defined, it is preferable to use the more specific subproperties Temporal Coverage and Spatial Coverage."@en ;
    dcterms:issued "2008-01-14"^^xsd:date ;
    rdfs:comment "The spatial or temporal topic of the resource, spatial applicability of the resource, or jurisdiction under which the resource is relevant."@en ;
    rdfs:isDefinedBy dcterms: ;
    rdfs:subPropertyOf dc:coverage ;
    skos:definition "El tema espacial o temporal del recurso, su aplicabilidad espacial o la jurisdicción bajo la cual es relevante."@es ;
    skos:prefLabel "Cobertura"@es .

dcterms:description a rdf:Property ;
    rdfs:label "Description"@en ;
    dcterms:description "Description may include but is not limited to: an abstract, a table of contents, a graphical representation, or a free-text account of the resource."@en ;
    dcterms:issued "2008-01-14"^^xsd:date ;
    rdfs:comment "An account of the resource."@en ;
    rdfs:isDefinedBy dcterms: ;
    rdfs:subPropertyOf dc:description ;
    skos:definition "Una descripción o relato del recurso."@es ;
    skos:prefLabel "Descripción"@es .

dcterms:format a rdf:Property ;
    rdfs:label "Format"@en ;
    dcam:rangeIncludes dcterms:Extent,
        dcterms:MediaType ;
    dcterms:description "Recommended practice is to use a controlled vocabulary where available. For example, for file formats one could use the list of Internet Media Types [[MIME](https://www.iana.org/assignments/media-types/media-types.xhtml)].  Examples of dimensions include size and duration."@en ;
    dcterms:issued "2008-01-14"^^xsd:date ;
    rdfs:comment "The file format, physical medium, or dimensions of the resource."@en ;
    rdfs:isDefinedBy dcterms: ;
    rdfs:subPropertyOf dc:format ;
    skos:definition "El tipo de archivo, el medio físico o las dimensiones con las que se presenta el recurso."@es ;
    skos:prefLabel "Formato"@es .

dcterms:rights a rdf:Property ;
    rdfs:label "Rights"@en ;
    dcam:rangeIncludes dcterms:RightsStatement ;
    dcterms:description "Typically, rights information includes a statement about various property rights associated with the resource, including intellectual property rights.  Recommended practice is to refer to a rights statement with a URI.  If this is not possible or feasible, a literal value (name, label, or short text) may be provided."@en ;
    dcterms:issued "2008-01-14"^^xsd:date ;
    rdfs:comment "Information about rights held in and over the resource."@en ;
    rdfs:isDefinedBy dcterms: ;
    rdfs:subPropertyOf dc:rights ;
    skos:definition "Información que describe los derechos de propiedad y de uso que se tienen sobre el recurso."@es ;
    skos:prefLabel "Derechos"@es .

dcterms:date a rdf:Property ;
    rdfs:label "Date"@en ;
    dcterms:description "Date may be used to express temporal information at any level of granularity.  Recommended practice is to express the date, date/time, or period of time according to ISO 8601-1 [[ISO 8601-1](https://www.iso.org/iso-8601-date-and-time-format.html)] or a published profile of the ISO standard, such as the W3C Note on Date and Time Formats [[W3CDTF](https://www.w3.org/TR/NOTE-datetime)] or the Extended Date/Time Format Specification [[EDTF](http://www.loc.gov/standards/datetime/)].  If the full date is unknown, month and year (YYYY-MM) or just year (YYYY) may be used. Date ranges may be specified using ISO 8601 period of time specification in which start and end dates are separated by a '/' (slash) character.  Either the start or end date may be missing."@en ;
    dcterms:issued "2008-01-14"^^xsd:date ;
    rdfs:comment "A point or period of time associated with an event in the lifecycle of the resource."@en ;
    rdfs:isDefinedBy dcterms: ;
    rdfs:range rdfs:Literal ;
    rdfs:subPropertyOf dc:date ;
    skos:definition "Un punto o período de tiempo asociado con un evento en el ciclo de vida del recurso."@es ;
    skos:prefLabel "Fecha"@es .

dcterms:relation a rdf:Property ;
    rdfs:label "Relation"@en ;
    dcterms:description "Recommended practice is to identify the related resource by means of a URI.  If this is not possible or feasible, a string conforming to a formal identification system may be provided."@en ;
    dcterms:issued "2008-01-14"^^xsd:date ;
    rdfs:comment "A related resource."@en ;
    rdfs:isDefinedBy dcterms: ;
    rdfs:subPropertyOf dc:relation ;
    skos:definition "Recurso que está vinculado o relacionado con otro, compartiendo temática, propósito o contenido."@es ;
    skos:prefLabel "Relación"@es .

dcterms: dcterms:modified "2012-06-14"^^xsd:date ;
    dcterms:publisher <http://purl.org/dc/aboutdcmi#DCMI> ;
    dcterms:title "DCMI Metadata Terms - other"@en .

